Update to ANF-Form. Missing typingok. Removed most of the metatheory.

src/dafny/Dot.dfy
@@ -45,20 +45,17 @@ function fresh_from(ids: seq<int>): int
 // Syntax
 // ------
 
-datatype tp = tp_sel(p: tm, L: nat, concrete: bool) | tp_rfn(base_tp: tp, self: nat, decls: list<decl>) | tp_and(and1: tp, and2: tp) | tp_or(or1: tp, or2: tp) | tp_top | tp_bot;
-datatype tm = tm_var(x: nat) | tm_new(y: nat, Tc: tp, init: list<def>, t': tm) | tm_sel(t: tm, l: nat) | tm_msel(o: tm, m: nat, a: tm) | tm_loc(loc: nat);
+datatype tp = tp_sel(p: pt, L: nat, concrete: bool) | tp_rfn(base_tp: tp, self: nat, decls: list<decl>) | tp_and(and1: tp, and2: tp) | tp_or(or1: tp, or2: tp) | tp_top | tp_bot;
+datatype pt = pt_var(x: nat) | pt_sel(p: pt, l: nat) |  pt_loc(loc: nat);
+datatype bd = bd_new(Tc: tp, init: list<def>) | bd_snd(o: pt, m: nat, a: pt) | bd_exe(ov: nat, mv: nat, t': tm);
+datatype tm = tm_path(p: pt) | tm_bind(y: nat, b: bd, t': tm);
 datatype decl = decl_tp(L: nat, S: tp, U: tp, concrete: bool) | decl_tm(l: nat, T: tp) | decl_mt(m: nat, P: tp, R: tp);
-datatype def = def_tm(l: nat, t: tm) | def_mt(m: nat, param: nat, body: tm);
+datatype def = def_tm(l: nat, v: pt) | def_mt(m: nat, param: nat, body: tm);
 datatype decls = decls_fin(decls: list<decl>) | decls_bot;
-
-predicate path(t: tm)
-{
-  t.tm_loc? || t.tm_var? || (t.tm_sel? && path(t.t))
-}
 
 predicate is_concrete(T: tp)
 {
-  (T.tp_sel? && T.concrete && path(T.p)) ||
+  (T.tp_sel? && T.concrete) ||
   (T.tp_rfn? && is_concrete(T.base_tp)) ||
   (T.tp_and? && is_concrete(T.and1) && is_concrete(T.and2)) ||
   T.tp_top?
@@ -79,11 +76,11 @@ function decl_label(d: decl): nat
 // ### Values ###
 predicate value(t: tm)
 {
-  t.tm_loc?
+  t.tm_path? && t.p.pt_loc?
 }
 predicate syn_value(t: tm)
 {
-  t.tm_loc? || t.tm_var?
+  t.tm_path? && (t.p.pt_loc? || t.p.pt_var?)
 }
 
 // ### Store ###
@@ -105,33 +102,51 @@ function def_method_lookup(m: nat, defs: seq<def>): option<pair<int, tm>>
   then (var i :| 0 <= i < |defs| && defs[i].def_mt? && defs[i].m==m; Some(P(defs[i].param, defs[i].body)))
   else None
 }
-function def_field_lookup(l: nat, defs: seq<def>): option<tm>
+function def_field_lookup(l: nat, defs: seq<def>): option<pt>
 {
   if (exists i :: 0 <= i < |defs| && defs[i].def_tm? && defs[i].l==l)
-  then (var i :| 0 <= i < |defs| && defs[i].def_tm? && defs[i].l==l; Some(defs[i].t))
+  then (var i :| 0 <= i < |defs| && defs[i].def_tm? && defs[i].l==l; Some(defs[i].v))
   else None
 }
 
 // ### Size ###
+function pt_size(p: pt): nat
+  ensures p.pt_sel? ==> pt_size(p)==1+pt_size(p.p);
+{
+  match p
+  case pt_var(x') => 1
+  case pt_loc(loc) => 1
+  case pt_sel(p1, l) => 1+pt_size(p1)
+}
+function bd_size(b: bd): nat
+  ensures b.bd_new? ==> bd_size(b)==1+tp_size(b.Tc)+defs_size(b.init);
+  ensures b.bd_new? ==> bd_size(b)>tp_size(b.Tc);
+  ensures b.bd_new? ==> bd_size(b)>defs_size(b.init);
+  ensures b.bd_snd? ==> bd_size(b)==1+pt_size(b.o)+pt_size(b.a);
+  ensures b.bd_snd? ==> bd_size(b)>pt_size(b.o);
+  ensures b.bd_snd? ==> bd_size(b)>pt_size(b.a);
+  ensures b.bd_exe? ==> bd_size(b)==1+tm_size(b.t');
+  ensures b.bd_exe? ==> bd_size(b)>tm_size(b.t');
+{
+  match b
+  case bd_new(Tc, init) => 1+tp_size(Tc)+defs_size(init)
+  case bd_snd(o, m, a) => 1+pt_size(o)+pt_size(a)
+  case bd_exe(ov, mv, t') => 1+tm_size(t')
+}
 function tm_size(t: tm): nat
-  ensures t.tm_new? ==> tm_size(t)==1+tp_size(t.Tc)+defs_size(t.init)+tm_size(t.t');
-  ensures t.tm_new? ==> tm_size(t)>tp_size(t.Tc);
-  ensures t.tm_new? ==> tm_size(t)>defs_size(t.init);
-  ensures t.tm_new? ==> tm_size(t)>tm_size(t.t');
-  ensures t.tm_sel? ==> tm_size(t)==1+tm_size(t.t);
-  ensures t.tm_msel? ==> tm_size(t)==1+tm_size(t.o)+tm_size(t.a);
-  ensures t.tm_msel? ==> tm_size(t)>tm_size(t.o);
+  ensures t.tm_path? ==> tm_size(t)==1+pt_size(t.p);
+  ensures t.tm_path? ==> tm_size(t)>pt_size(t.p);
+  ensures t.tm_bind? ==> tm_size(t)==1+bd_size(t.b)+tm_size(t.t');
+  ensures t.tm_bind? ==> tm_size(t)>bd_size(t.b);
+  ensures t.tm_bind? ==> tm_size(t)>tm_size(t.t');
 {
   match t
-  case tm_var(x') => 1
-  case tm_new(y, Tc, init, t1) => 1+tp_size(Tc)+defs_size(init)+tm_size(t1)
-  case tm_sel(t1, l) => 1+tm_size(t1)
-  case tm_msel(o, m, a) => 1+tm_size(o)+tm_size(a)
-  case tm_loc(loc) => 1
+  case tm_path(p) => 1+pt_size(p)
+  case tm_bind(x, b, t') => 1+bd_size(b)+tm_size(t')
 }
 function tp_size(T: tp): nat
-  ensures T.tp_sel? ==> tp_size(T)==1+tm_size(T.p);
-  ensures T.tp_sel? ==> tp_size(T)>tm_size(T.p);
+  ensures T.tp_sel? ==> tp_size(T)==1+pt_size(T.p);
+  ensures T.tp_sel? ==> tp_size(T)>pt_size(T.p);
   ensures T.tp_rfn? ==> tp_size(T)==1+tp_size(T.base_tp)+decls_size(T.decls);
   ensures T.tp_rfn? ==> tp_size(T)>tp_size(T.base_tp);
   ensures T.tp_rfn? ==> tp_size(T)>decls_size(T.decls);
@@ -141,7 +156,7 @@ function tp_size(T: tp): nat
   ensures T.tp_or? ==> tp_size(T)>tp_size(T.or1);
 {
   match T
-  case tp_sel(p, L, concrete) => 1+tm_size(p)
+  case tp_sel(p, L, concrete) => 1+pt_size(p)
   case tp_rfn(base_tp, self, decls) => 1+tp_size(base_tp)+decls_size(decls)
   case tp_and(and1, and2) => 1+tp_size(and1)+tp_size(and2)
   case tp_or(or1, or2) => 1+tp_size(or1)+tp_size(or2)
@@ -149,13 +164,13 @@ function tp_size(T: tp): nat
   case tp_bot => 1
 }
 function def_size(d: def): nat
-  ensures d.def_tm? ==> def_size(d)==1+tm_size(d.t);
-  ensures d.def_tm? ==> def_size(d)>tm_size(d.t);
+  ensures d.def_tm? ==> def_size(d)==1+pt_size(d.v);
+  ensures d.def_tm? ==> def_size(d)>pt_size(d.v);
   ensures d.def_mt? ==> def_size(d)==1+tm_size(d.body);
   ensures d.def_mt? ==> def_size(d)>tm_size(d.body);
 {
   match d
-  case def_tm(l, t1) => 1+tm_size(t1)
+  case def_tm(l, v1) => 1+pt_size(v1)
   case def_mt(m, param, body) => 1+tm_size(body)
 }
 function decl_size(d: decl): nat
@@ -191,60 +206,76 @@ function decls_size(decls: list<decl>): nat
 }
 
 // ### Substitution ###
-function tm_subst(x: nat, v: tm, t: tm): tm
+function pt_subst(x: nat, v: pt, p: pt): pt
+  decreases pt_size(p), p;
+  ensures v.pt_var? ==> pt_size(p)==pt_size(pt_subst(x, v, p));
+  ensures !pt_fn(x, p) ==> pt_subst(x, v, p)==p;
+{
+  match p
+  case pt_var(x') => if x'==x then v else p
+  case pt_sel(p1, l) => pt_sel(pt_subst(x, v, p1), l)
+  case pt_loc(loc) => p
+}
+function bd_subst(x: nat, v: pt, b: bd): bd
+  decreases bd_size(b), b;
+  ensures v.pt_var? ==> bd_size(b)==bd_size(bd_subst(x, v, b));
+  ensures !bd_fn(x, b) ==> bd_subst(x, v, b)==b;
+{
+  match b
+  case bd_new(Tc, init) => bd_new(tp_subst(x, v, Tc), defs_subst(x, v, init))
+  case bd_snd(o, m, a) => bd_snd(pt_subst(x, v, o), m, pt_subst(x, v, a))
+  case bd_exe(ov, mv, t') => bd_exe(ov, mv, tm_subst(x, v, t'))
+}
+function tm_subst(x: nat, v: pt, t: tm): tm
   decreases tm_size(t), t;
-  ensures v.tm_var? ==> tm_size(t)==tm_size(tm_subst(x, v, t));
-  ensures path(v) && path(t) ==> path(tm_subst(x, v, t));
+  ensures v.pt_var? ==> tm_size(t)==tm_size(tm_subst(x, v, t));
   ensures !tm_fn(x, t) ==> tm_subst(x, v, t)==t;
 {
   match t
-  case tm_var(x') => if x'==x then v else t
-  case tm_new(y, Tc, init, t1) =>
+  case tm_path(p) => tm_path(pt_subst(x, v, p))
+  case tm_bind(y, b, t1) =>
     if !tm_fn(x, t) then t else
-    if y==x then tm_new(y, tp_subst(x, v, Tc), init, t1) else
-    var y' := fresh_from([x]+tm_vars(v)+tm_vars(t));
-    var init' := defs_subst(y, tm_var(y'), init);
-    var t1' := tm_subst(y, tm_var(y'), t1);
-    tm_new(y', tp_subst(x, v, Tc), defs_subst(x, v, init'), tm_subst(x, v, t1'))
-  case tm_sel(t1, l) => tm_sel(tm_subst(x, v, t1), l)
-  case tm_msel(o, m, a) => tm_msel(tm_subst(x, v, o), m, tm_subst(x, v, a))
-  case tm_loc(loc) => t
+    if y==x then (if b.bd_new? then tm_bind(y, bd_new(tp_subst(x, v, b.Tc), b.init), t1) else tm_bind(y, bd_subst(x, v, b), t1)) else
+    var y' := fresh_from([x]+pt_vars(v)+tm_vars(t));
+    var b' := bd_subst(y, pt_var(y'), b);
+    var t1' := tm_subst(y, pt_var(y'), t1);
+    tm_bind(y', bd_subst(x, v, b'), tm_subst(x, v, t1'))
 }
-function tp_subst(x: nat, v: tm, T: tp): tp
+function tp_subst(x: nat, v: pt, T: tp): tp
   decreases tp_size(T), T;
-  ensures v.tm_var? ==> tp_size(T)==tp_size(tp_subst(x, v, T));
+  ensures v.pt_var? ==> tp_size(T)==tp_size(tp_subst(x, v, T));
   ensures !tp_fn(x, T) ==> tp_subst(x, v, T)==T;
 {
   match T
-  case tp_sel(p, L, concrete) => tp_sel(tm_subst(x, v, p), L, concrete)
+  case tp_sel(p, L, concrete) => tp_sel(pt_subst(x, v, p), L, concrete)
   case tp_rfn(base_tp, self, decls) =>
     if !tp_fn(x, T) then T else
     if self==x then tp_rfn(tp_subst(x, v, base_tp), self, decls) else
-    var self' := fresh_from([x]+tm_vars(v)+tp_vars(T));
-    var decls' := decls_subst(self, tm_var(self'), decls);
+    var self' := fresh_from([x]+pt_vars(v)+tp_vars(T));
+    var decls' := decls_subst(self, pt_var(self'), decls);
     tp_rfn(tp_subst(x, v, base_tp), self', decls_subst(x, v, decls'))
   case tp_and(and1, and2) => tp_and(tp_subst(x, v, and1), tp_subst(x, v, and2))
   case tp_or(or1, or2) => tp_or(tp_subst(x, v, or1), tp_subst(x, v, or2))
   case tp_top => T
   case tp_bot => T
 }
-function def_subst(x: nat, v: tm, d: def): def
+function def_subst(x: nat, v: pt, d: def): def
   decreases def_size(d), d;
-  ensures v.tm_var? ==> def_size(d)==def_size(def_subst(x, v, d));
+  ensures v.pt_var? ==> def_size(d)==def_size(def_subst(x, v, d));
   ensures !def_fn(x, d) ==> def_subst(x, v, d)==d;
 {
   match d
-  case def_tm(l, t1) => def_tm(l, tm_subst(x, v, t1))
+  case def_tm(l, v1) => def_tm(l, pt_subst(x, v, v1))
   case def_mt(m, param, body) =>
     if !def_fn(x, d) then d else
     if param==x then d else
-    var param' := fresh_from([x]+tm_vars(v)+def_vars(d));
-    var body' := tm_subst(param, tm_var(param'), body);
+    var param' := fresh_from([x]+pt_vars(v)+def_vars(d));
+    var body' := tm_subst(param, pt_var(param'), body);
     def_mt(m, param', tm_subst(x, v, body'))
 }
-function decl_subst(x: nat, v: tm, d: decl): decl
+function decl_subst(x: nat, v: pt, d: decl): decl
   decreases decl_size(d), d;
-  ensures v.tm_var? ==> decl_size(d)==decl_size(decl_subst(x, v, d));
+  ensures v.pt_var? ==> decl_size(d)==decl_size(decl_subst(x, v, d));
   ensures !decl_fn(x, d) ==> decl_subst(x, v, d)==d;
 {
   match d
@@ -252,18 +283,18 @@ function decl_subst(x: nat, v: tm, d: decl): decl
   case decl_tm(l, T) => decl_tm(l, tp_subst(x, v, T))
   case decl_mt(m, P, R) => decl_mt(m, tp_subst(x, v, P), tp_subst(x, v, R))
 }
-function defs_subst(x: nat, v: tm, defs: list<def>): list<def>
+function defs_subst(x: nat, v: pt, defs: list<def>): list<def>
   decreases defs_size(defs), defs;
-  ensures v.tm_var? ==> defs_size(defs)==defs_size(defs_subst(x, v, defs));
+  ensures v.pt_var? ==> defs_size(defs)==defs_size(defs_subst(x, v, defs));
   ensures !defs_fn(x, defs) ==> defs_subst(x, v, defs)==defs;
 {
   match defs
   case Nil => Nil
   case Cons(head, tail) => Cons(def_subst(x, v, head), defs_subst(x, v, tail))
 }
-function decls_subst(x: nat, v: tm, decls: list<decl>): list<decl>
+function decls_subst(x: nat, v: pt, decls: list<decl>): list<decl>
   decreases decls_size(decls), decls;
-  ensures v.tm_var? ==> decls_size(decls)==decls_size(decls_subst(x, v, decls));
+  ensures v.pt_var? ==> decls_size(decls)==decls_size(decls_subst(x, v, decls));
   ensures !decls_fn(x, decls) ==> decls_subst(x, v, decls)==decls;
 {
   match decls
@@ -274,23 +305,43 @@ function decls_subst(x: nat, v: tm, decls: list<decl>): list<decl>
 // ### Free variables ###
 // fn(x, A) <==> x appears free in A
 
+predicate pt_fn(x: nat, p: pt)
+  ensures pt_fn(x, p) ==> x in pt_vars(p);
+  decreases p;
+{
+  match p
+  case pt_var(x') => x'==x
+  case pt_sel(p1, l) => pt_fn(x, p1)
+  case pt_loc(loc) => false
+}
+
+predicate bd_fn(x: nat, b: bd)
+  ensures bd_fn(x, b) ==> x in bd_vars(b);
+  decreases b;
+{
+  match b
+  case bd_new(Tc, init) => tp_fn(x, Tc) || defs_fn(x, init)
+  case bd_snd(o, m, a) => pt_fn(x, o) || pt_fn(x, a)
+  case bd_exe(ov, mv, t') => tm_fn(x, t')
+}
+
 predicate tm_fn(x: nat, t: tm)
   ensures tm_fn(x, t) ==> x in tm_vars(t);
   decreases t;
 {
   match t
-  case tm_var(x') => x'==x
-  case tm_new(y, Tc, init, t') => tp_fn(x, Tc) || (y!=x && (defs_fn(x, init) || tm_fn(x, t')))
-  case tm_sel(t1, l) => tm_fn(x, t1)
-  case tm_msel(o, m, a) => tm_fn(x, o) || tm_fn(x, a)
-  case tm_loc(loc) => false
+  case tm_path(p) => pt_fn(x, p)
+  case tm_bind(y, b, t') =>
+    if (y==x) then (if b.bd_new? then tp_fn(x, b.Tc) else bd_fn(x, b)) else
+    bd_fn(x, b) && tm_fn(x, t')
 }
+
 predicate tp_fn(x: nat, T: tp)
   ensures tp_fn(x, T) ==> x in tp_vars(T);
   decreases T;
 {
   match T
-  case tp_sel(p, L, concrete) => tm_fn(x, p)
+  case tp_sel(p, L, concrete) => pt_fn(x, p)
   case tp_rfn(base_tp, self, decls) => tp_fn(x, base_tp) || (self!=x && decls_fn(x, decls))
   case tp_and(and1, and2) => tp_fn(x, and1) || tp_fn(x, and2)
   case tp_or(or1, or2) => tp_fn(x, or1) || tp_fn(x, or2)
@@ -302,7 +353,7 @@ predicate def_fn(x: nat, d: def)
   decreases d;
 {
   match d
-  case def_tm(l, t1) => tm_fn(x, t1)
+  case def_tm(l, v1) => pt_fn(x, v1)
   case def_mt(m, param, body) => param!=x && tm_fn(x, body)
 }
 predicate decl_fn(x: nat, d: decl)
@@ -328,21 +379,38 @@ predicate decls_fn(x: nat, decls: list<decl>)
 }
 
 // ### Variables ###
+
+function pt_vars(p: pt): seq<int>
+  ensures forall x :: x in pt_vars(p) ==> x>=0;
+{
+  match p
+  case pt_var(x') => [x']
+  case pt_sel(p1, l) => pt_vars(p1)
+  case pt_loc(loc) => []
+}
+
+function bd_vars(b: bd): seq<int>
+  ensures forall x :: x in bd_vars(b) ==> x>=0;
+{
+  match b
+  case bd_new(Tc, init) => tp_vars(Tc)+defs_vars(init)
+  case bd_snd(o, m, a) => pt_vars(o)+pt_vars(a)
+  case bd_exe(ov, mv, t') => tm_vars(t')
+}
+
 function tm_vars(t: tm): seq<int>
   ensures forall x :: x in tm_vars(t) ==> x>=0;
 {
   match t
-  case tm_var(x') => [x']
-  case tm_new(y, Tc, init, t') => [y]+tp_vars(Tc)+defs_vars(init)+tm_vars(t')
-  case tm_sel(t1, l) => tm_vars(t1)
-  case tm_msel(o, m, a) => tm_vars(o)+tm_vars(a)
-  case tm_loc(loc) => []
+  case tm_path(p) => pt_vars(p)
+  case tm_bind(y, b, t') => [y]+bd_vars(b)+tm_vars(t')
 }
+
 function tp_vars(T: tp): seq<int>
   ensures forall x :: x in tp_vars(T) ==> x>=0;
 {
   match T
-  case tp_sel(p, L, concrete) => tm_vars(p)
+  case tp_sel(p, L, concrete) => pt_vars(p)
   case tp_rfn(base_tp, self, decls) => tp_vars(base_tp)+[self]+decls_vars(decls)
   case tp_and(and1, and2) => tp_vars(and1)+tp_vars(and2)
   case tp_or(or1, or2) => tp_vars(or1)+tp_vars(or2)
@@ -353,7 +421,7 @@ function def_vars(d: def): seq<int>
   ensures forall x :: x in def_vars(d) ==> x>=0;
 {
   match d
-  case def_tm(l, t1) => tm_vars(t1)
+  case def_tm(l, v1) => pt_vars(v1)
   case def_mt(m, param, body) => [param]+tm_vars(body)
 }
 function decl_vars(d: decl): seq<int>
@@ -382,32 +450,48 @@ function decls_vars(decls: list<decl>): seq<int>
 }
 
 // ### Reduction ###
+function pt_step(p: pt, s: store): option<pair<pt, store>>
+{
+  /* sel */
+  if (p.pt_sel? && p.p.pt_loc? && p.p.loc < |s.m| &&
+      def_field_lookup(p.l, store_lookup(p.p.loc, s)).Some?)
+  then Some(P(def_field_lookup(p.l, store_lookup(p.p.loc, s)).get, s))
+  /* sel-c */
+  else if (p.pt_sel? && pt_step(p.p, s).Some?)
+  then Some(P(pt_sel(pt_step(p.p, s).get.fst, p.l), pt_step(p.p, s).get.snd))
+  else None
+}
+
 function step(t: tm, s: store): option<pair<tm, store>>
 {
-  /* msel */
-  if (t.tm_msel? && t.o.tm_loc? && value(t.a) && t.o.loc < |s.m| &&
-     def_method_lookup(t.m, store_lookup(t.o.loc, s)).Some?)
-  then Some(P(tm_subst(def_method_lookup(t.m, store_lookup(t.o.loc, s)).get.fst,
-                       t.a,
-                       def_method_lookup(t.m, store_lookup(t.o.loc, s)).get.snd),
-              s))
-  /* msel1 */
-  else if (t.tm_msel? && step(t.o, s).Some?)
-  then Some(P(tm_msel(step(t.o, s).get.fst, t.m, t.a), step(t.o, s).get.snd))
-  /* msel2 */
-  else if (t.tm_msel? && value(t.o) && step(t.a, s).Some?)
-  then Some(P(tm_msel(t.o, t.m, step(t.a, s).get.fst), step(t.a, s).get.snd))
-  /* sel */
-  else if (t.tm_sel? && t.t.tm_loc? && t.t.loc < |s.m| &&
-           def_field_lookup(t.l, store_lookup(t.t.loc, s)).Some?)
-  then Some(P(def_field_lookup(t.l, store_lookup(t.t.loc, s)).get, s))
-  /* sel1 */
-  else if (t.tm_sel? && step(t.t, s).Some?)
-  then Some(P(tm_sel(step(t.t, s).get.fst, t.l), step(t.t, s).get.snd))
+  if (t.tm_path? && pt_step(t.p, s).Some?)
+  then Some(P(tm_path(pt_step(t.p, s).get.fst), pt_step(t.p, s).get.snd))
   /* new */
-  else if (t.tm_new?)
-  then Some(P(tm_subst(t.y, tm_loc(|s.m|), t.t'),
-              Store(s.m+[P(t.Tc, lst2seq(defs_subst(t.y, tm_loc(|s.m|), t.init)))])))
+  else if (t.tm_bind? && t.b.bd_new?)
+  then Some(P(tm_subst(t.y, pt_loc(|s.m|), t.t'),
+              Store(s.m+[P(t.b.Tc, lst2seq(defs_subst(t.y, pt_loc(|s.m|), t.b.init)))])))
+  /* snd */
+  else if (t.tm_bind? && t.b.bd_snd? && t.b.o.pt_loc? && value(tm_path(t.b.a)) && t.b.o.loc < |s.m| &&
+     def_method_lookup(t.b.m, store_lookup(t.b.o.loc, s)).Some?)
+  then Some(P(tm_bind(t.y,
+                      bd_exe(t.b.o.loc, t.b.m,
+                             tm_subst(def_method_lookup(t.b.m, store_lookup(t.b.o.loc, s)).get.fst,
+                                      t.b.a,
+                                      def_method_lookup(t.b.m, store_lookup(t.b.o.loc, s)).get.snd)),
+                      t.t'),
+              s))
+  /* snd-c-obj */
+  else if (t.tm_bind? && t.b.bd_snd? && pt_step(t.b.o, s).Some?)
+  then Some(P(tm_bind(t.y, bd_snd(pt_step(t.b.o, s).get.fst, t.b.m, t.b.a), t.t'), pt_step(t.b.o, s).get.snd))
+  /* snd-c-arg */
+  else if (t.tm_bind? && t.b.bd_snd? && value(tm_path(t.b.o)) && pt_step(t.b.a, s).Some?)
+  then Some(P(tm_bind(t.y, bd_snd(t.b.o, t.b.m, pt_step(t.b.a, s).get.fst), t.t'), pt_step(t.b.a, s).get.snd))
+  /* exe */
+  else if (t.tm_bind? && t.b.bd_exe? && value(t.b.t'))
+  then Some(P(tm_subst(t.y, t.b.t'.p, t.t'), s))
+  /* exe-c */
+  else if (t.tm_bind? && t.b.bd_exe? && step(t.b.t', s).Some?)
+  then Some(P(tm_bind(t.y, bd_exe(t.b.ov, t.b.mv, step(t.b.t', s).get.fst), t.t'), step(t.b.t', s).get.snd))
   else None
 }
 
@@ -460,8 +544,9 @@ ghost method lemma_mstep_trans'(t1: tm, s1: store, t2: tm, s2: store, t3: tm, s3
 // ### Congruence Lemmas ###
 
 ghost method lemma_mstep_sel(o: tm, l: nat, o': tm, s: store, s': store, oi: nat)
+  requires o.tm_path? && o'.tm_path?;
   requires mstep(o, s, o', s', oi);
-  ensures mstep(tm_sel(o, l), s, tm_sel(o', l), s', oi);
+  ensures mstep(tm_path(pt_sel(o.p, l)), s, tm_path(pt_sel(o'.p, l)), s', oi);
   decreases oi;
 {
   if (oi>0) {
@@ -470,7 +555,8 @@ ghost method lemma_mstep_sel(o: tm, l: nat, o': tm, s: store, s': store, oi: nat
 }
 
 ghost method lemma_sel_irred__o_mstep_irred(o: tm, l: nat, t': tm, s: store, s': store, i: nat) returns (o': tm, so': store, oi: nat)
-  requires mstep(tm_sel(o, l), s, t', s', i);
+  requires o.tm_path?;
+  requires mstep(tm_path(pt_sel(o.p, l)), s, t', s', i);
   requires irred(t', s');
   ensures oi<=i && mstep(o, s, o', so', oi) && irred(o', so');
   decreases i;
@@ -481,7 +567,7 @@ ghost method lemma_sel_irred__o_mstep_irred(o: tm, l: nat, t': tm, s: store, s':
     oi := 0;
   } else {
     assert step(o, s).Some?;
-    lemma_mstep_trans'(tm_sel(o, l), s, tm_sel(step(o, s).get.fst, l), step(o, s).get.snd, t', s', 1, i);
+    lemma_mstep_trans'(tm_path(pt_sel(o.p, l)), s, tm_path(pt_sel(step(o, s).get.fst.p, l)), step(o, s).get.snd, t', s', 1, i);
     var o'', so'', oi' := lemma_sel_irred__o_mstep_irred(step(o, s).get.fst, l, t', step(o, s).get.snd, s', i-1);
     lemma_mstep_trans(o, s, step(o, s).get.fst, step(o, s).get.snd, o'', so'', 1, oi');
     o' := o'';
@@ -684,43 +770,14 @@ function decls_or(Ds1: decls, Ds2: decls): decls
 
 // ### Typing-Related Judgments ###
 
-predicate typing(n: nat, ctx: context, s: store, t: tm, T: tp)
+predicate typing(n: nat, ctx: context, s: store, p: pt, T: tp)
   decreases n;
 {
-  match t
-  case tm_var(x) => context_lookup(ctx, x)==Some(T)
-  case tm_new(y_, Tc, init_, t'_) =>
-    var y := fresh_from(dom(ctx)+tm_vars(t));
-    var init := defs_subst(y_, tm_var(y), init_);
-    var t' := tm_subst(y_, tm_var(y), t'_);
-    n>0 && is_concrete(Tc) &&
-    exists Ds:decls :: Ds.decls_fin? &&
-    wfe_type(n-1, ctx, s, Tc) &&
-    expansion(n-1, ctx, s, y, Tc, Ds) && 
-    wf_init(n-1, false, context_extend(ctx, y, Tc), s, lst2seq(Ds.decls), lst2seq(init)) &&
-    !tp_fn(y, T) &&
-    exists T' :: typing(n-1, context_extend(ctx, y, Tc), s, t', T') &&
-    subtype(n-1, context_extend(ctx, y, Tc), s, T', T)
-  case tm_sel(t, l) =>
-    n>0 && field_membership(n-1, ctx, s, t, l, T)
-  case tm_msel(o, m, a) =>
-    n>0 && exists S, T' :: method_membership(n-1, ctx, s, o, m, S, T) &&
-    typing(n-1, ctx, s, a, T') &&
-    subtype(n-1, ctx, s, T', S)
-  case tm_loc(loc) => loc < |s.m| && store_lookup_type(loc, s)==T
-}
-predicate wf_init(n: nat, already_in_store: bool, ctx: context, s: store, decls: seq<decl>, defs: seq<def>)
-  decreases n;
-{
-  var p:nat := fresh_in_context(ctx);
-  n>0 && forall d :: d in decls ==> (
-  if (d.decl_tp?) then subtype(n-1, ctx, s, d.S, d.U)
-  else if (d.decl_tm?) then exists def :: def in defs && def.def_tm? && def.l==d.l && (if already_in_store then value(def.t) else syn_value(def.t)) &&
-                            exists T :: typing(n-1, ctx, s, def.t, T) && subtype(n-1, ctx, s, T, d.T)
-  else if (d.decl_mt?) then exists def :: def in defs && def.def_mt? && def.m==d.m &&
-                            exists T' :: typing(n-1, context_extend(ctx, p, d.P), s, tm_subst(def.param, tm_var(p), def.body), T') &&
-                                         subtype(n-1, context_extend(ctx, p, d.P), s, T', d.R)
-  else false)
+  match p
+  case pt_var(x) => context_lookup(ctx, x)==Some(T)
+  case pt_sel(p1, l) =>
+    n>0 && field_membership(n-1, ctx, s, p1, l, T)
+  case pt_loc(loc) => loc < |s.m| && store_lookup_type(loc, s)==T
 }
 predicate wf_decl(n: nat, ctx: context, s: store, d: decl)
   decreases n;
@@ -742,10 +799,9 @@ predicate wf_type(n: nat, ctx: context, s: store, T: tp)
   match T
   case tp_rfn(T', z_, Ds_) =>
     var z:= fresh_in_context(ctx);
-    var Ds := decls_subst(z_, tm_var(z), Ds_);
+    var Ds := decls_subst(z_, pt_var(z), Ds_);
     n>0 && wf_type(n-1, ctx, s, T') && wf_decls(n-1, context_extend(ctx, z, T), s, lst2seq(Ds))
   case tp_sel(p, L, concrete) =>
-    path(p) &&
     n>0 && exists S, U :: type_membership(n-1, ctx, s, p, L, concrete, S, U)
   case tp_and(T1, T2) => n>0 && wf_type(n-1, ctx, s, T1) && wf_type(n-1, ctx, s, T2)
   case tp_or(T1, T2) => n>0 && wf_type(n-1, ctx, s, T1) && wf_type(n-1, ctx, s, T2)
@@ -757,35 +813,33 @@ predicate wfe_type(n: nat, ctx: context, s: store, T: tp)
 {
   n>0 && wf_type(n-1, ctx, s, T) && exists Ds :: expansion(n-1, ctx, s, 0, T, Ds)
 }
-predicate membership(n: nat, ctx: context, s: store, t: tm, l: nat, d: decl)
+predicate membership(n: nat, ctx: context, s: store, p: pt, l: nat, d: decl)
   decreases n;
 {
   var z:nat := fresh_in_context(ctx);
   decl_label(d)==l &&
-  n>0 && exists T, T' :: typing(n-1, ctx, s, t, T') &&
-  subtype(n-1, ctx, s, T', T) &&
+  n>0 && exists T :: typing(n-1, ctx, s, p, T) &&
   exists Ds ::
   expansion(n-1, ctx, s, z, T, Ds) &&
   ((Ds.decls_fin? &&
-     ((path(t) && T'==T && exists d' :: d' in lst2seq(Ds.decls) && d==decl_subst(z, t, d')) ||
-      (!path(t) && d in lst2seq(Ds.decls) && !decl_fn(z, d)))) ||
+    exists d' :: d' in lst2seq(Ds.decls) && d==decl_subst(z, p, d')) ||
    (Ds.decls_bot? && decl_bot(d)))
 }
-predicate field_membership(n: nat, ctx: context, s: store, t: tm, l: nat, T: tp)
+predicate field_membership(n: nat, ctx: context, s: store, p: pt, l: nat, T: tp)
   decreases n;
 {
-  n>0 && membership(n-1, ctx, s, t, l, decl_tm(l, T))
+  n>0 && membership(n-1, ctx, s, p, l, decl_tm(l, T))
 }
-predicate method_membership(n: nat, ctx: context, s: store, t: tm, m: nat, P: tp, R: tp)
+predicate method_membership(n: nat, ctx: context, s: store, p: pt, m: nat, P: tp, R: tp)
   decreases n;
 {
-  n>0 && exists d :: membership(n-1, ctx, s, t, m, d) &&
+  n>0 && exists d :: membership(n-1, ctx, s, p, m, d) &&
   d.decl_mt? && d.m==m && d.P==P && d.R==R
 }
-predicate type_membership(n: nat, ctx: context, s: store, t: tm, L: nat, concrete: bool, S: tp, U: tp)
+predicate type_membership(n: nat, ctx: context, s: store, p: pt, L: nat, concrete: bool, S: tp, U: tp)
   decreases n;
 {
-  n>0 && exists d :: membership(n-1, ctx, s, t, L, d) &&
+  n>0 && exists d :: membership(n-1, ctx, s, p, L, d) &&
   d.decl_tp? && d.L==L && d.concrete==concrete && d.S==S && d.U==U
 }
 predicate m_decl_seq_sorted(m: seq<pair<tp, decls>>)
@@ -811,7 +865,7 @@ predicate expansion_iter(n: nat, m: seq<pair<tp, decls>>, ctx: context, s: store
   case tp_rfn(T', z', Ds') =>
     n>0 &&
     exists DsT' :: expansion_iter(n-1, m, ctx, s, z, T', DsT') &&
-    exists rfn_decls :: rfn_decls==decl_seq_sort(lst2seq(decls_subst(z', tm_var(z), Ds'))) &&
+    exists rfn_decls :: rfn_decls==decl_seq_sort(lst2seq(decls_subst(z', pt_var(z), Ds'))) &&
     Ds==decls_and(decls_fin(seq2lst(rfn_decls)), DsT')
   case tp_sel(p, L, concrete) =>
     (lookup(T, m).Some? && lookup(T, m).get==Ds) || 
@@ -866,13 +920,12 @@ predicate decls_sub(n: nat, ctx: context, s: store, Ds1: decls, Ds2: decls)
      case decls_bot => false
      case decls_fin(s2) => n>0 && decls_fin_sub(n-1, ctx, s, lst2seq(s1), lst2seq(s2)))
 }
-predicate path_red(ctx: context, s: store, p1: tm, p2: tm)
+predicate path_red(ctx: context, s: store, p1: pt, p2: pt)
 {
-  path(p1) && path(p2) && (
-  (p1.tm_sel? && p1.t.tm_loc? && p2.tm_loc? && p1.t.loc < |s.m| &&
-   def_field_lookup(p1.l, store_lookup(p1.t.loc, s)).Some? &&
-   p2==def_field_lookup(p1.l, store_lookup(p1.t.loc, s)).get) ||
-  (p1.tm_sel? && p2.tm_sel? && p1.l==p2.l && path_red(ctx, s, p1.t, p2.t)))
+  (p1.pt_sel? && p1.p.pt_loc? && p2.pt_loc? && p1.p.loc < |s.m| &&
+   def_field_lookup(p1.l, store_lookup(p1.p.loc, s)).Some? &&
+   p2==def_field_lookup(p1.l, store_lookup(p1.p.loc, s)).get) ||
+  (p1.pt_sel? && p2.pt_sel? && p1.l==p2.l && path_red(ctx, s, p1.p, p2.p))
 }
 
 predicate subtype(n: nat, ctx: context, s: store, S: tp, T: tp)
@@ -885,7 +938,7 @@ predicate subtype(n: nat, ctx: context, s: store, S: tp, T: tp)
   /* bot-<: */  (S.tp_bot? && wfe_type(n-1, ctx, s, T)) ||
   /* <:-rfn */  (T.tp_rfn? && wfe_type(n-1, ctx, s, T) && subtype(n-1, ctx, s, S, T.base_tp) &&
                  exists Ds' :: expansion(n-1, ctx, s, self, S, Ds') &&
-                 exists rfn_decls :: rfn_decls==decl_seq_sort(lst2seq(decls_subst(T.self, tm_var(self), T.decls))) &&
+                 exists rfn_decls :: rfn_decls==decl_seq_sort(lst2seq(decls_subst(T.self, pt_var(self), T.decls))) &&
                  decls_sub(n-1, context_extend(ctx, self, S), s, decls_fin(seq2lst(rfn_decls)), Ds')) ||
   /* rfn-<: */  (S.tp_rfn? && wfe_type(n-1, ctx, s, S) && subtype(n-1, ctx, s, S.base_tp, T)) ||
   /* <:-sel */  (T.tp_sel? &&
@@ -904,27 +957,23 @@ predicate subtype(n: nat, ctx: context, s: store, S: tp, T: tp)
                  subtype(n-1, ctx, s, S, tp_sel(p, T.L, T.concrete))))
 }
 
-predicate typing'(ctx: context, s: store, t: tm, T: tp)
+predicate typing'(ctx: context, s: store, p: pt, T: tp)
 {
-  exists n:nat :: typing(n, ctx, s, t, T)
-}
-predicate wf_init'(already_in_store: bool, ctx: context, s: store, decls: seq<decl>, defs: seq<def>)
-{
-  exists n:nat :: wf_init(n, already_in_store, ctx, s, decls, defs)
+  exists n:nat :: typing(n, ctx, s, p, T)
 }
 predicate wfe_type'(ctx: context, s: store, T: tp)
 {
   exists n:nat :: wfe_type(n, ctx, s, T)
 }
-predicate membership'(ctx: context, s: store, t: tm, l: nat, d: decl)
+predicate membership'(ctx: context, s: store, t: pt, l: nat, d: decl)
 {
   exists n:nat :: membership(n, ctx, s, t, l, d)
 }
-predicate field_membership'(ctx: context, s: store, t: tm, l: nat, T: tp)
+predicate field_membership'(ctx: context, s: store, t: pt, l: nat, T: tp)
 {
   exists n:nat :: field_membership(n, ctx, s, t, l, T)
 }
-predicate method_membership'(ctx: context, s: store, t: tm, m: nat, P: tp, R: tp)
+predicate method_membership'(ctx: context, s: store, t: pt, m: nat, P: tp, R: tp)
 {
   exists n:nat :: method_membership(n, ctx, s, t, m, P, R)
 }
@@ -943,17 +992,11 @@ predicate subtype'(ctx: context, s: store, S: tp, T: tp)
 }
 
 // ### Properties about typing-related judgments ###
-function typing_n(ctx: context, s: store, t: tm, T: tp): nat
+function typing_n(ctx: context, s: store, t: pt, T: tp): nat
   requires typing'(ctx, s, t, T);
   ensures typing(typing_n(ctx, s, t, T), ctx, s, t, T);
 {
   var n:nat :| typing(n, ctx, s, t, T); n
-}
-function wf_init_n(already_in_store: bool, ctx: context, s: store, decls: seq<decl>, defs: seq<def>): nat
-  requires wf_init'(already_in_store, ctx, s, decls, defs);
-  ensures wf_init(wf_init_n(already_in_store, ctx, s, decls, defs), already_in_store, ctx, s, decls, defs);
-{
-  var n:nat :| wf_init(n, already_in_store, ctx, s, decls, defs); n
 }
 function wfe_type_n(ctx: context, s: store, T: tp): nat
   requires wfe_type'(ctx, s, T);
@@ -961,13 +1004,13 @@ function wfe_type_n(ctx: context, s: store, T: tp): nat
 {
   var n:nat :| wfe_type(n, ctx, s, T); n
 }
-function field_membership_n(ctx: context, s: store, t: tm, l: nat, T: tp): nat
+function field_membership_n(ctx: context, s: store, t: pt, l: nat, T: tp): nat
   requires field_membership'(ctx, s, t, l, T);
   ensures field_membership(field_membership_n(ctx, s, t, l, T), ctx, s, t, l, T);
 {
   var n:nat :| field_membership(n, ctx, s, t, l, T); n
 }
-function method_membership_n(ctx: context, s: store, t: tm, m: nat, P: tp, R: tp): nat
+function method_membership_n(ctx: context, s: store, t: pt, m: nat, P: tp, R: tp): nat
   requires method_membership'(ctx, s, t, m, P, R);
   ensures method_membership(method_membership_n(ctx, s, t, m, P, R), ctx, s, t, m, P, R);
 {
@@ -986,7 +1029,7 @@ function subtype_n(ctx: context, s: store, S: tp, T: tp): nat
   var n:nat :| subtype(n, ctx, s, S, T); n
 }
 
-ghost method lemma_typing_monotonic_plus(m: nat, n: nat, ctx: context, s: store, t: tm, T: tp)
+ghost method lemma_typing_monotonic_plus(m: nat, n: nat, ctx: context, s: store, t: pt, T: tp)
   requires m<=n;
   requires typing(m, ctx, s, t, T);
   ensures typing(n, ctx, s, t, T);
@@ -998,71 +1041,17 @@ ghost method lemma_typing_monotonic_plus(m: nat, n: nat, ctx: context, s: store,
     lemma_typing_monotonic_plus(m+1, n, ctx, s, t, T);
   }
 }
-ghost method lemma_typing_monotonic(n: nat, ctx: context, s: store, t: tm, T: tp)
+ghost method lemma_typing_monotonic(n: nat, ctx: context, s: store, t: pt, T: tp)
   requires typing(n, ctx, s, t, T);
   ensures typing(n+1, ctx, s, t, T);
 {
-  if (t.tm_var?) {
+  if (t.pt_var?) {
     assert typing(n+1, ctx, s, t, T);
-  } else if (t.tm_new?) {
+  } else if (t.pt_sel?) {
     if (n>0) {
-      var y := fresh_from(dom(ctx)+tm_vars(t));
-      var init := defs_subst(t.y, tm_var(y), t.init);
-      var t' := tm_subst(t.y, tm_var(y), t.t');
-      var Ds:decls :| Ds.decls_fin? &&
-      wfe_type(n-1, ctx, s, t.Tc) &&
-      expansion(n-1, ctx, s, y, t.Tc, Ds) && 
-      wf_init(n-1, false, context_extend(ctx, y, t.Tc), s, lst2seq(Ds.decls), lst2seq(init)) &&
-      !tp_fn(y, T) &&
-      exists T' :: typing(n-1, context_extend(ctx, y, t.Tc), s, t', T') &&
-      subtype(n-1, context_extend(ctx, y, t.Tc), s, T', T);
-
-      var T':tp :| typing(n-1, context_extend(ctx, y, t.Tc), s, t', T') &&
-      subtype(n-1, context_extend(ctx, y, t.Tc), s, T', T);
-
-      lemma_wfe_type_monotonic(n-1, ctx, s, t.Tc);
-      lemma_expansion_monotonic(n-1, ctx, s, y, t.Tc, Ds); 
-      lemma_wf_init_monotonic(n-1, false, context_extend(ctx, y, t.Tc), s, lst2seq(Ds.decls), lst2seq(init));
-      lemma_typing_monotonic(n-1, context_extend(ctx, y, t.Tc), s, t', T');
-      lemma_subtype_monotonic(n-1, context_extend(ctx, y, t.Tc), s, T', T);
-    }
-  } else if (t.tm_sel?) {
-    if (n>0) {
-      lemma_field_membership_monotonic(n-1, ctx, s, t.t, t.l, T);
-    }
-  } else if (t.tm_msel?) {
-    if (n>0) {
-      var S, T' :| method_membership(n-1, ctx, s, t.o, t.m, S, T) &&
-      typing(n-1, ctx, s, t.a, T') &&
-      subtype(n-1, ctx, s, T', S);
-
-      lemma_method_membership_monotonic(n-1, ctx, s, t.o, t.m, S, T);
-      lemma_typing_monotonic(n-1, ctx, s, t.a, T');
-      lemma_subtype_monotonic(n-1, ctx, s, T', S);
-
-      assert method_membership(n, ctx, s, t.o, t.m, S, T) &&
-      typing(n, ctx, s, t.a, T') &&
-      subtype(n, ctx, s, T', S);
-
-      helper_assert_exists_method_membership(n, ctx, s, t, T, S, T');
+      lemma_field_membership_monotonic(n-1, ctx, s, t.p, t.l, T);
     }
   }
-}
-ghost method helper_assert_exists_method_membership(n: nat, ctx: context, s: store, t: tm, T: tp, S: tp, T': tp)
-  requires t.tm_msel?;
-  requires method_membership(n, ctx, s, t.o, t.m, S, T) &&
-      typing(n, ctx, s, t.a, T') &&
-      subtype(n, ctx, s, T', S);
-  ensures exists S, T' :: method_membership(n, ctx, s, t.o, t.m, S, T) &&
-      typing(n, ctx, s, t.a, T') &&
-      subtype(n, ctx, s, T', S);
-{
-}
-ghost method lemma_wf_init_monotonic(n: nat, already_in_store: bool, ctx: context, s: store, decls: seq<decl>, defs: seq<def>)
-  requires wf_init(n, already_in_store, ctx, s, decls, defs);
-  ensures wf_init(n+1, already_in_store, ctx, s, decls, defs);
-{
-  assume wf_init(n+1, already_in_store, ctx, s, decls, defs); // TODO
 }
 ghost method lemma_wfe_type_monotonic(n: nat, ctx: context, s: store, T: tp)
   requires wfe_type(n, ctx, s, T);
@@ -1070,13 +1059,13 @@ ghost method lemma_wfe_type_monotonic(n: nat, ctx: context, s: store, T: tp)
 {
   assume wfe_type(n+1, ctx, s, T); // TODO
 }
-ghost method lemma_field_membership_monotonic(n: nat, ctx: context, s: store, t: tm, l: nat, T: tp)
+ghost method lemma_field_membership_monotonic(n: nat, ctx: context, s: store, t: pt, l: nat, T: tp)
   requires field_membership(n, ctx, s, t, l, T);
   ensures field_membership(n+1, ctx, s, t, l, T);
 {
   assume field_membership(n+1, ctx, s, t, l, T); // TODO
 }
-ghost method lemma_method_membership_monotonic(n: nat, ctx: context, s: store, t: tm, m: nat, P: tp, R: tp)
+ghost method lemma_method_membership_monotonic(n: nat, ctx: context, s: store, t: pt, m: nat, P: tp, R: tp)
   requires method_membership(n, ctx, s, t, m, P, R);
   ensures method_membership(n+1, ctx, s, t, m, P, R);
 {
@@ -1138,940 +1127,9 @@ predicate store_extends<A>(s': store, s: store)
 {
   |s.m|<=|s'.m| && forall l:nat :: l < |s.m| ==> s.m[l]==s'.m[l]
 }
-predicate store_well_typed1(s: store, loc: nat, y: nat, Tc: tp, init: seq<def>)
-{
-    exists n:nat :: n>0 &&
-    is_concrete(Tc) &&
-    exists Ds:decls :: Ds.decls_fin? &&
-    wfe_type(n-1, Context([]), s, Tc) &&
-    expansion(n-1, Context([]), s, y, Tc, Ds) && 
-    wf_init(n-1, true, Context([]), s, lst2seq(decls_subst(y, tm_loc(loc), Ds.decls)), init) &&
-    tp_closed(Tc) &&
-    forall d :: d in init ==> def_closed(d)
-}
-predicate store_well_typed(s: store)
-{
-  forall l:nat :: l < |s.m| ==> store_well_typed1(s, l, fresh_from([]), store_lookup_type(l, s), store_lookup(l, s))
-}
-predicate env_well_typed(ctx: context, s: store)
-{
-  store_well_typed(s) && forall x:nat :: context_lookup(ctx, x).Some? ==> wfe_type'(ctx, s, context_lookup(ctx, x).get)
-}
-ghost method lemma_store_invariance_typing(n: nat, ctx: context, s: store, s': store, t: tm, T: tp)
-  requires store_extends(s', s);
-  requires typing(n, ctx, s, t, T);
-  ensures typing(n, ctx, s', t, T);
-  decreases n;
-{
-  if (t.tm_sel?) {
-    lemma_store_invariance_membership(n-2, ctx, s, s', t.t, t.l, decl_tm(t.l, T));
-  } else if (t.tm_msel?) {
-    var S, T' :| method_membership(n-1, ctx, s, t.o, t.m, S, T) &&
-    typing(n-1, ctx, s, t.a, T') &&
-    subtype(n-1, ctx, s, T', S);
-    lemma_store_invariance_membership(n-2, ctx, s, s', t.o, t.m, decl_mt(t.m, S, T));
-    lemma_store_invariance_typing(n-1, ctx, s, s', t.a, T');
-    lemma_store_invariance_subtype(n-1, ctx, s, s', T', S);
-    assert method_membership(n-1, ctx, s', t.o, t.m, S, T) &&
-    typing(n-1, ctx, s', t.a, T') &&
-    subtype(n-1, ctx, s', T', S);
-    helper_assert_exists_method_membership(n-1, ctx, s', t, T, S, T');
-  } else if (t.tm_new?) {
-    var y := fresh_from(dom(ctx)+tm_vars(t));
-    var init := defs_subst(t.y, tm_var(y), t.init);
-    var t' := tm_subst(t.y, tm_var(y), t.t');
-    var Ds:decls, T' :| Ds.decls_fin? &&
-    wfe_type(n-1, ctx, s, t.Tc) &&
-    expansion(n-1, ctx, s, y, t.Tc, Ds) && 
-    wf_init(n-1, false, context_extend(ctx, y, t.Tc), s, lst2seq(Ds.decls), lst2seq(init)) &&
-    !tp_fn(y, T) &&
-    typing(n-1, context_extend(ctx, y, t.Tc), s, t', T') &&
-    subtype(n-1, context_extend(ctx, y, t.Tc), s, T', T);
-    lemma_store_invariance_wfe_type(n-1, ctx, s, s', t.Tc);
-    lemma_store_invariance_expansion(n-1, ctx, s, s', y, t.Tc, Ds); 
-    lemma_store_invariance_wf_init(n-1, false, context_extend(ctx, y, t.Tc), s, s', lst2seq(Ds.decls), lst2seq(init));
-    lemma_store_invariance_typing(n-1, context_extend(ctx, y, t.Tc), s, s', t', T');
-    lemma_store_invariance_subtype(n-1, context_extend(ctx, y, t.Tc), s, s', T', T);
-    assert Ds.decls_fin? &&
-    wfe_type(n-1, ctx, s', t.Tc) &&
-    expansion(n-1, ctx, s', y, t.Tc, Ds) && 
-    wf_init(n-1, false, context_extend(ctx, y, t.Tc), s', lst2seq(Ds.decls), lst2seq(init)) &&
-    !tp_fn(y, T) &&
-    typing(n-1, context_extend(ctx, y, t.Tc), s', t', T') &&
-    subtype(n-1, context_extend(ctx, y, t.Tc), s', T', T);
-    helper_assert_exists_new(n-1, ctx, s', t, y, init, t', T, Ds, T');
-  } else {
-  }
-}
-ghost method helper_assert_exists_new(n: nat, ctx: context, s: store, t: tm,  y: nat, init: list<def>, t': tm, T: tp, Ds: decls, T': tp)
-  requires t.tm_new?;
-  requires context_lookup(ctx, y).None?;
-  requires Ds.decls_fin? &&
-    wfe_type(n, ctx, s, t.Tc) &&
-    expansion(n, ctx, s, y, t.Tc, Ds) && 
-    wf_init(n, false, context_extend(ctx, y, t.Tc), s, lst2seq(Ds.decls), lst2seq(init)) &&
-    !tp_fn(y, T) &&
-    typing(n, context_extend(ctx, y, t.Tc), s, t', T') &&
-    subtype(n, context_extend(ctx, y, t.Tc), s, T', T);
-  ensures exists Ds:decls, T' :: Ds.decls_fin? &&
-    wfe_type(n, ctx, s, t.Tc) &&
-    expansion(n, ctx, s, y, t.Tc, Ds) && 
-    wf_init(n, false, context_extend(ctx, y, t.Tc), s, lst2seq(Ds.decls), lst2seq(init)) &&
-    !tp_fn(y, T) &&
-    typing(n, context_extend(ctx, y, t.Tc), s, t', T') &&
-    subtype(n, context_extend(ctx, y, t.Tc), s, T', T);
-{
-}
-ghost method lemma_store_invariance_membership(n: nat, ctx: context, s: store, s': store, t: tm, l: nat, d: decl)
-  requires store_extends(s', s);
-  requires membership(n, ctx, s, t, l, d);
-  ensures membership(n, ctx, s', t, l, d);
-{
-  assume membership(n, ctx, s', t, l, d); // TODO
-}
-ghost method lemma_store_invariance_subtype(n: nat, ctx: context, s: store, s': store, S: tp, T: tp)
-  requires store_extends(s', s);
-  requires subtype(n, ctx, s, S, T);
-  ensures subtype(n, ctx, s', S, T);
-{
-  assume subtype(n, ctx, s', S, T); // TODO
-}
-ghost method lemma_store_invariance_wfe_type(n: nat, ctx: context, s: store, s': store, T: tp)
-  requires store_extends(s', s);
-  requires wfe_type(n, ctx, s, T);
-  ensures wfe_type(n, ctx, s', T);
-{
-  assume wfe_type(n, ctx, s', T); // TODO
-}
-ghost method lemma_store_invariance_expansion(n: nat, ctx: context, s: store, s': store, z: nat, T: tp, Ds: decls)
-  requires store_extends(s', s);
-  requires expansion(n, ctx, s, z, T, Ds);
-  ensures expansion(n, ctx, s', z, T, Ds);
-{
-  assume expansion(n, ctx, s', z, T, Ds);
-}
-ghost method lemma_store_invariance_wf_init(n: nat, already_in_store: bool, ctx: context, s: store, s': store, decls: seq<decl>, defs: seq<def>)
-  requires store_extends(s', s);
-  requires wf_init(n, already_in_store, ctx, s, decls, defs);
-  ensures wf_init(n, already_in_store, ctx, s', decls, defs);
-{
-  assume wf_init(n, already_in_store, ctx, s', decls, defs);
-}
-ghost method lemma_store_invariance_well_typed1(s: store, s': store, loc: nat, y: nat, Tc: tp, init: seq<def>)
-  requires store_extends(s', s);
-  requires store_well_typed1(s, loc, y, Tc, init);
-  ensures store_well_typed1(s', loc, y, Tc, init);
-{
-  var n:nat, Ds:decls :| n>0 &&
-    is_concrete(Tc) &&
-    Ds.decls_fin? &&
-    wfe_type(n-1, Context([]), s, Tc) &&
-    expansion(n-1, Context([]), s, y, Tc, Ds) && 
-    wf_init(n-1, true, Context([]), s, lst2seq(decls_subst(y, tm_loc(loc), Ds.decls)), init);
-  lemma_store_invariance_wfe_type(n-1, Context([]), s, s', Tc);
-  lemma_store_invariance_expansion(n-1, Context([]), s, s', y, Tc, Ds); 
-  lemma_store_invariance_wf_init(n-1, true, Context([]), s, s', lst2seq(decls_subst(y, tm_loc(loc), Ds.decls)), init);
-  assert n>0 &&
-    is_concrete(Tc) &&
-    Ds.decls_fin? &&
-    wfe_type(n-1, Context([]), s', Tc) &&
-    expansion(n-1, Context([]), s', y, Tc, Ds) && 
-    wf_init(n-1, true, Context([]), s', lst2seq(decls_subst(y, tm_loc(loc), Ds.decls)), init);
-  helper_assert_exists_store_well_typed1(s', loc, y, Tc, init, n, Ds);
-}
-ghost method helper_assert_exists_store_well_typed1(s: store, loc: nat, y: nat, Tc: tp, init: seq<def>, n: nat, Ds: decls)
-  requires n>0 &&
-    is_concrete(Tc) &&
-    Ds.decls_fin? &&
-    wfe_type(n-1, Context([]), s, Tc) &&
-    expansion(n-1, Context([]), s, y, Tc, Ds) && 
-    wf_init(n-1, true, Context([]), s, lst2seq(decls_subst(y, tm_loc(loc), Ds.decls)), init);
-  ensures exists n:nat, Ds:decls :: n>0 &&
-    is_concrete(Tc) &&
-    Ds.decls_fin? &&
-    wfe_type(n-1, Context([]), s, Tc) &&
-    expansion(n-1, Context([]), s, y, Tc, Ds) && 
-    wf_init(n-1, true, Context([]), s, lst2seq(decls_subst(y, tm_loc(loc), Ds.decls)), init);
-{
-}
-
-ghost method lemma_store_extends_well_typed(s: store, s': store, Tc: tp, init: seq<def>)
-  requires store_well_typed(s);
-  requires s'==Store(s.m+[P(Tc, init)]);
-  requires store_well_typed1(s', |s.m|, fresh_from([]), Tc, init);
-  ensures store_extends(s', s);
-  ensures store_well_typed(s');
-{
-  forall (l:nat | l < |s'.m|)
-  ensures store_well_typed1(s', l, fresh_from([]), store_lookup_type(l, s'), store_lookup(l, s'));
-  {
-    if (l == |s.m|) {
-    } else {
-      assert l < |s.m|;
-      var initl := store_lookup(l, s);
-      var Tcl := store_lookup_type(l, s); 
-      assert store_well_typed1(s, l, fresh_from([]), Tcl, initl);
-      assert store_lookup(l, s') == initl;
-      assert store_lookup_type(l, s') == Tcl;
-      lemma_store_invariance_well_typed1(s, s', l, fresh_from([]), Tcl, initl);
-    }
-  }
-}
-
-ghost method lemma_free_after_tm_subst(x: nat, y_: nat, y: nat, t_: tm)
-  requires x!=y_;
-  requires tm_fn(x, t_);
-  ensures tm_fn(x, tm_subst(y_, tm_var(y), t_));
-  decreases tm_size(t_);
-{
-  if (t_.tm_var?) {
-  } else if (t_.tm_loc?) {
-  } else if (t_.tm_sel?) {
-  } else if (t_.tm_msel?) {
-  } else if (t_.tm_new?) {
-    if (!tm_fn(y_, t_)) {
-    } else if (t_.y==y_) {
-      assert tm_subst(y_, tm_var(y), t_) == tm_new(t_.y, tp_subst(y_, tm_var(y), t_.Tc), t_.init, t_.t');
-      if (tp_fn(x, t_.Tc)) {
-        lemma_free_after_tp_subst(x, y_, y, t_.Tc);
-      }
-    } else {
-      var y' := fresh_from([y_]+tm_vars(tm_var(y))+tm_vars(t_));
-      var init' := defs_subst(t_.y, tm_var(y'), t_.init);
-      var t1' := tm_subst(t_.y, tm_var(y'), t_.t');
-      assert tm_subst(y_, tm_var(y), t_) == tm_new(y', tp_subst(y_, tm_var(y), t_.Tc), defs_subst(y_, tm_var(y), init'), tm_subst(y_, tm_var(y), t1'));
-      if (tp_fn(x, t_.Tc)) {
-       lemma_free_after_tp_subst(x, y_, y, t_.Tc);
-      } else if (defs_fn(x, t_.init)) {
-        lemma_free_after_defs_subst(x, t_.y, y', t_.init);
-        assert defs_fn(x, init');
-        lemma_free_after_defs_subst(x, y_, y, init');
-        assert defs_fn(x, defs_subst(y_, tm_var(y), init'));
-        assert tm_fn(x, tm_new(y', tp_subst(y_, tm_var(y), t_.Tc), defs_subst(y_, tm_var(y), init'), tm_subst(y_, tm_var(y), t1')));
-        assert tm_fn(x, tm_subst(y_, tm_var(y), t_));
-      } else if (tm_fn(x, t_.t')) {
-        lemma_free_after_tm_subst(x, t_.y, y', t_.t');
-        lemma_free_after_tm_subst(x, y_, y, t1');
-      } else {
-      }
-    }
-  } else {
-  }
-}
-ghost method lemma_free_after_tp_subst(x: nat, y_: nat, y: nat, T_: tp)
-  requires x!=y_;
-  requires tp_fn(x, T_);
-  ensures tp_fn(x, tp_subst(y_, tm_var(y), T_));
-{
-  assume tp_fn(x, tp_subst(y_, tm_var(y), T_)); // TODO
-}
-ghost method lemma_free_after_defs_subst(x: nat, y_: nat, y: nat, init_: list<def>)
-  requires x!=y_;
-  requires defs_fn(x, init_);
-  ensures defs_fn(x, defs_subst(y_, tm_var(y), init_));
-{
-  assume defs_fn(x, defs_subst(y_, tm_var(y), init_)); // TODO
-}
-
-
-ghost method lemma_free_in_context_typing(x:nat, n: nat, ctx: context, s: store, t: tm, T: tp)
-  requires tm_fn(x, t);
-  requires typing(n, ctx, s, t, T);
-  ensures context_lookup(ctx, x).Some?;
-{
-  if (t.tm_var?) {
-  } else if (t.tm_loc?) {
-  } else if (t.tm_sel?) {
-    assert membership(n-2, ctx, s, t.t, t.l, decl_tm(t.l, T));
-    var To :| typing(n-3, ctx, s, t.t, To);
-    lemma_free_in_context_typing(x, n-3, ctx, s, t.t, To);
-  } else if (t.tm_msel?) {
-    var S, T' :| method_membership(n-1, ctx, s, t.o, t.m, S, T) &&
-    typing(n-1, ctx, s, t.a, T') &&
-    subtype(n-1, ctx, s, T', S);
-    assert membership(n-2, ctx, s, t.o, t.m, decl_mt(t.m, S, T));
-    var To :| typing(n-3, ctx, s, t.o, To);
-    assert tm_fn(x, t.o) || tm_fn(x, t.a);
-    if (tm_fn(x, t.o)) {
-      lemma_free_in_context_typing(x, n-3, ctx, s, t.o, To);
-    }
-    if (tm_fn(x, t.a)) {
-      lemma_free_in_context_typing(x, n-1, ctx, s, t.a, T');
-    }
-  } else if (t.tm_new?) {
-    var y := fresh_from(dom(ctx)+tm_vars(t));
-    var init := defs_subst(t.y, tm_var(y), t.init);
-    var t' := tm_subst(t.y, tm_var(y), t.t');
-    if (tp_fn(x, t.Tc)) {
-     assert wfe_type(n-1, ctx, s, t.Tc);
-     lemma_free_in_context_wfe_type(x, n-1, ctx, s, t.Tc);
-    } else if (tm_fn(x, t.t')) {
-      lemma_free_after_tm_subst(x, t.y, y, t.t');
-      assert tm_fn(x, t');
-      var T' :| typing(n-1, context_extend(ctx, y, t.Tc), s, t', T');
-      lemma_free_in_context_typing(x, n-1, context_extend(ctx, y, t.Tc), s, t', T');
-    } else if (defs_fn(x, t.init)) {
-      lemma_free_after_defs_subst(x, t.y, y, t.init);
-      assert defs_fn(x, init);
-      assume context_lookup(ctx, x).Some?; // TODO (really!)
-    }
-  } else {
-  }
-}
-ghost method lemma_free_in_context_wfe_type(x: nat, n: nat, ctx: context, s: store, T: tp)
-  requires tp_fn(x, T);
-  requires wfe_type(n, ctx, s, T);
-  ensures context_lookup(ctx, x).Some?;
-  ensures wfe_type(n, ctx, s, T);
-{
-  assume context_lookup(ctx, x).Some?; // TODO (really!)
-}
-ghost method lemma_wfe_type_not_in_context(x: nat, n: nat, ctx: context, st: store, T: tp)
-  requires context_lookup(ctx, x).None?;
-  requires wfe_type(n, ctx, st, T);
-  ensures wfe_type(n, ctx, st, T);
-  ensures !tp_fn(x, T);
-{
-  if (tp_fn(x, T)) {
-    lemma_free_in_context_wfe_type(x, n, ctx, st, T);
-    assert false;
-  }
-}
-
-ghost method lemma_typing__wfe(n: nat, ctx: context, s: store, t: tm, T: tp) returns (n': nat)
-  requires typing(n, ctx, s, t, T);
-  requires env_well_typed(ctx, s);
-  ensures wfe_type(n', ctx, s, T);
-{
-  assume exists n'':nat :: wfe_type(n'', ctx, s, T); // TODO
-  var n'':nat :| wfe_type(n'', ctx, s, T);
-  n' := n'';
-}
-ghost method lemma_subtype__wfe(n: nat, ctx: context, s: store, S: tp, T: tp) returns (n': nat)
-  requires subtype(n, ctx, s, S, T);
-  requires env_well_typed(ctx, s);
-  ensures wfe_type(n', ctx, s, S);
-  ensures wfe_type(n', ctx, s, T);
-{
-  assume exists n'':nat :: wfe_type(n'', ctx, s, S) && wfe_type(n'', ctx, s, T); // TODO
-  var n'':nat :| wfe_type(n'', ctx, s, S) && wfe_type(n'', ctx, s, T);
-  n' := n'';
-}
-
-ghost method corollary_typable_empty__closed(n: nat, s: store, t: tm, T: tp)
-  requires typing(n, Context([]), s, t, T);
-  requires env_well_typed(Context([]), s);
-  ensures tm_closed(t);
-  ensures tp_closed(T);
-{
-  forall (x: nat)
-    ensures !tm_fn(x, t) && !tp_fn(x, T);
-  {
-    if (tm_fn(x, t)) {
-      lemma_free_in_context_typing(x, n, Context([]), s, t, T);
-      assert context_lookup(Context([]), x).Some?;
-      assert false;
-    }
-    assert !tm_fn(x, t);
-    if (tp_fn(x, T)) {
-      var nwfe := lemma_typing__wfe(n, Context([]), s, t, T);
-      lemma_free_in_context_wfe_type(x, nwfe, Context([]), s, T);
-      assert false;
-    }
-    assert !tp_fn(x, T);
-  }
-}
-ghost method lemma_not_fn__subst_idem(x: nat, s: tm, T: tp)
-  requires !tp_fn(x, T);
-  ensures tp_subst(x, s, T)==T;
-{
-}
-
-ghost method lemma_context_invariance(n: nat, ctx: context, ctx': context, s: store, t: tm, T: tp)
-  requires typing(n, ctx, s, t, T);
-  requires forall x:nat :: tm_fn(x, t) ==> context_lookup(ctx, x) == context_lookup(ctx', x);
-  ensures typing(n, ctx', s, t, T);
-  decreases t;
-{
-  assume typing(n, ctx', s, t, T); // TODO (really!)
-}
-
-ghost method lemma_decl_bot__subst_idem(x: nat, s: tm, d: decl)
+ghost method lemma_decl_bot__subst_idem(x: nat, s: pt, d: decl)
   requires decl_bot(d);
   ensures decl_bot(decl_subst(x, s, d));
   ensures decl_eq(d, decl_subst(x, s, d));
 {
-}
-ghost method lemma_path_subst2(x: nat, s: tm, z: nat, o: tm, t: tm)
-  requires x!=z;
-  requires value(s);
-  requires path(o);
-  ensures tm_subst(x, s, tm_subst(z, o, t))==tm_subst(z, tm_subst(x, s, o), tm_subst(x, s, t));
-{
-  match t {
-  case tm_var(x') =>
-  case tm_new(y, Tc, init, t1) =>
-    // TODO, but not important for decls
-    assume tm_subst(x, s, tm_subst(z, o, t))==tm_subst(z, tm_subst(x, s, o), tm_subst(x, s, t));
-  case tm_sel(t1, l) =>
-  case tm_msel(o, m, a) =>
-  case tm_loc(loc) =>
-  }
-}
-ghost method lemma_tp_subst2(x: nat, s: tm, z: nat, o: tm, T: tp)
-  requires x!=z;
-  requires value(s);
-  requires path(o);
-  ensures tp_subst(x, s, tp_subst(z, o, T))==tp_subst(z, tm_subst(x, s, o), tp_subst(x, s, T)); // TODO: maybe this is only true up to alpha-equivalence? need to be more cautious in subst.
-{
-  match T {
-  case tp_sel(p, L, concrete) =>
-    lemma_path_subst2(x, s, z, o, p);
-  case tp_rfn(base_tp, self, decls) =>
-    if (!tp_fn(x, tp_subst(z, o, T))) {
-      assert tp_subst(x, s, tp_subst(z, o, T))==tp_subst(z, o, T);
-      if (!tp_fn(z, T)) {
-      } else if (self==z) {
-        // TODO
-        assume tp_subst(x, s, tp_subst(z, o, T))==tp_subst(z, tm_subst(x, s, o), tp_subst(x, s, T));
-      } else {
-        assert tp_fn(z, T);
-        // TODO
-        assume tp_subst(x, s, tp_subst(z, o, T))==tp_subst(z, tm_subst(x, s, o), tp_subst(x, s, T));
-      }
-    } else if (self==x) {
-       // TODO
-       assume tp_subst(x, s, tp_subst(z, o, T))==tp_subst(z, tm_subst(x, s, o), tp_subst(x, s, T));
-    } else {
-       // TODO
-       assume tp_subst(x, s, tp_subst(z, o, T))==tp_subst(z, tm_subst(x, s, o), tp_subst(x, s, T));
-    }
-  case tp_and(and1, and2) =>
-  case tp_or(or1, or2) =>
-  case tp_top =>
-  case tp_bot =>
-  }
-}
-ghost method lemma_decl_subst2(x: nat, s: tm, z: nat, o: tm, d: decl)
-  requires x!=z;
-  requires value(s);
-  requires path(o);
-  ensures decl_subst(x, s, decl_subst(z, o, d))==decl_subst(z, tm_subst(x, s, o), decl_subst(x, s, d));  
-{
-  match d {
-  case decl_tp(L, S, U, concrete) =>
-    lemma_tp_subst2(x, s, z, o, S);
-    lemma_tp_subst2(x, s, z, o, U);
-  case decl_tm(l, T) =>
-    lemma_tp_subst2(x, s, z, o, T);
-  case decl_mt(m, P, R) =>
-    lemma_tp_subst2(x, s, z, o, P);
-    lemma_tp_subst2(x, s, z, o, R);
-  }
-}
-
-ghost method lemma_decl_fn_subst(z: nat, x: nat, s: tm, d: decl)
-  requires !decl_fn(z, d);
-  requires value(s);
-  ensures !decl_fn(z, decl_subst(x, s, d));
-{
-  assert !tm_fn(z, s);
-  assume !decl_fn(z, decl_subst(x, s, d)); // TODO
-}
-
-ghost method lemma_not_path_subst(x: nat, s: tm, t: tm)
-  requires value(s);
-  requires !path(t);
-  ensures !path(tm_subst(x, s, t));
-{
-}
-ghost method lemma_path_subst(x: nat, s: tm, t: tm)
-  requires value(s);
-  requires path(t);
-  ensures path(tm_subst(x, s, t));
-{
-}
-ghost method lemma_fresh_equiv_membership_sel(z: nat, z': nat, ctx: context, st: store, x: nat, s: tm, t: tm, To: tp, To': tp, Ds': decls, d: decl, maxn: nat) returns (Ds'': decls)
-  requires t.tm_sel?;
-  requires decl_label(decl_subst(x, s, d))==t.l;
-  requires typing(maxn, ctx, st, tm_subst(x, s, t.t), tp_subst(x, s, To'));
-  requires subtype(maxn, ctx, st, tp_subst(x, s, To'), tp_subst(x, s, To));
-  requires expansion(maxn, ctx, st, z, tp_subst(x, s, To), Ds');
-  requires ((Ds'.decls_fin? &&
-     ((path(tm_subst(x, s, t.t)) && tp_subst(x, s, To')==tp_subst(x, s, To) && exists d'' :: d'' in lst2seq(Ds'.decls) && decl_subst(x, s, d)==decl_subst(z, tm_subst(x, s, t.t), d'')) ||
-      (!path(tm_subst(x, s, t.t)) && decl_subst(x, s, d) in lst2seq(Ds'.decls) && !decl_fn(z, decl_subst(x, s, d))))) ||
-   (Ds'.decls_bot? && decl_bot(decl_subst(x, s, d))));
-  requires value(s);
-  requires context_lookup(ctx, x).None?;
-  requires env_well_typed(ctx, st);
-  requires context_lookup(ctx, z).None?;
-  requires context_lookup(ctx, z').None?;
-  ensures expansion(maxn, ctx, st, z', tp_subst(x, s, To), Ds'');
-  ensures ((Ds''.decls_fin? &&
-     ((path(tm_subst(x, s, t.t)) && tp_subst(x, s, To')==tp_subst(x, s, To) && exists d'' :: d'' in lst2seq(Ds''.decls) && decl_subst(x, s, d)==decl_subst(z', tm_subst(x, s, t.t), d'')) ||
-      (!path(tm_subst(x, s, t.t)) && decl_subst(x, s, d) in lst2seq(Ds''.decls) && !decl_fn(z', decl_subst(x, s, d))))) ||
-   (Ds''.decls_bot? && decl_bot(decl_subst(x, s, d))));
-{
-  assume exists Ds''' ::  expansion(maxn, ctx, st, z', tp_subst(x, s, To), Ds''') &&
-   ((Ds'''.decls_fin? &&
-     ((path(tm_subst(x, s, t.t)) && tp_subst(x, s, To')==tp_subst(x, s, To) && exists d'' :: d'' in lst2seq(Ds'''.decls) && decl_subst(x, s, d)==decl_subst(z', tm_subst(x, s, t.t), d'')) ||
-      (!path(tm_subst(x, s, t.t)) && decl_subst(x, s, d) in lst2seq(Ds'''.decls) && !decl_fn(z', decl_subst(x, s, d))))) ||
-   (Ds'''.decls_bot? && decl_bot(decl_subst(x, s, d))));
-   var Ds''' :| expansion(maxn, ctx, st, z', tp_subst(x, s, To), Ds''') &&
-   ((Ds'''.decls_fin? &&
-     ((path(tm_subst(x, s, t.t)) && tp_subst(x, s, To')==tp_subst(x, s, To) && exists d'' :: d'' in lst2seq(Ds'''.decls) && decl_subst(x, s, d)==decl_subst(z', tm_subst(x, s, t.t), d'')) ||
-      (!path(tm_subst(x, s, t.t)) && decl_subst(x, s, d) in lst2seq(Ds'''.decls) && !decl_fn(z', decl_subst(x, s, d))))) ||
-   (Ds'''.decls_bot? && decl_bot(decl_subst(x, s, d))));
-   Ds'' := Ds''';
-}
-ghost method lemma_assert_membership(maxn: nat, ctx: context, st: store, x: nat, s: tm, t: tm, d: decl, To: tp, To': tp, z': nat, Ds'': decls)
-  requires t.tm_sel?;
-  requires decl_label(d)==t.l;
-  requires typing(maxn, ctx, st, tm_subst(x, s, t.t), tp_subst(x, s, To'));
-  requires subtype(maxn, ctx, st, tp_subst(x, s, To'), tp_subst(x, s, To));
-  requires z'==fresh_in_context(ctx);
-  requires expansion(maxn, ctx, st, z', tp_subst(x, s, To), Ds'');
-  requires ((Ds''.decls_fin? &&
-     ((path(tm_subst(x, s, t.t)) && tp_subst(x, s, To')==tp_subst(x, s, To) && exists d'' :: d'' in lst2seq(Ds''.decls) && decl_subst(x, s, d)==decl_subst(z', tm_subst(x, s, t.t), d'')) ||
-      (!path(tm_subst(x, s, t.t)) && decl_subst(x, s, d) in lst2seq(Ds''.decls) && !decl_fn(z', decl_subst(x, s, d))))) ||
-   (Ds''.decls_bot? && decl_bot(decl_subst(x, s, d))));
-  requires decl_label(decl_subst(x, s, d))==tm_subst(x, s, t).l;
-  ensures membership(maxn+1, ctx, st, tm_subst(x, s, t.t), tm_subst(x, s, t).l, decl_subst(x, s, d));
-{
-}
-ghost method lemma_assert_membership'(maxn: nat, n': nat, ctx: context, st: store, x: nat, s: tm, o: tm, l: nat, d: decl, To: tp, To': tp, z': nat, Ds'': decls)
-  requires decl_label(d)==l;
-  requires typing(maxn, ctx, st, tm_subst(x, s, o), tp_subst(x, s, To'));
-  requires subtype(maxn, ctx, st, tp_subst(x, s, To'), tp_subst(x, s, To));
-  requires z'==fresh_in_context(ctx);
-  requires expansion(maxn, ctx, st, z', tp_subst(x, s, To), Ds'');
-  requires ((Ds''.decls_fin? &&
-     ((path(tm_subst(x, s, o)) && tp_subst(x, s, To')==tp_subst(x, s, To) && exists d'' :: d'' in lst2seq(Ds''.decls) && decl_subst(x, s, d)==decl_subst(z', tm_subst(x, s, o), d'')) ||
-      (!path(tm_subst(x, s, o)) && decl_subst(x, s, d) in lst2seq(Ds''.decls) && !decl_fn(z', decl_subst(x, s, d))))) ||
-   (Ds''.decls_bot? && decl_bot(decl_subst(x, s, d))));
-  ensures decl_label(decl_subst(x, s, d))==l;
-  requires n'==maxn+1;
-  ensures membership(n', ctx, st, tm_subst(x, s, o), l, decl_subst(x, s, d));
-{
-}
-// NOTE: no narrowing yet
-ghost method lemma_case_sel_substitution_preserves_typing(ctx: context, st: store, x: nat, s: tm, S: tp, ns: nat, t: tm, T: tp, nt: nat) returns (n': nat)
-  requires t.tm_sel?;
-  requires value(s);
-  requires typing(ns, Context([]), st, s, S);
-  requires context_lookup(ctx, x).None?;
-  requires env_well_typed(ctx, st);
-  requires typing(nt+1, context_extend(ctx, x, S), st, t, T);
-  ensures typing(n', ctx, st, tm_subst(x, s, t), tp_subst(x, s, T));
-  decreases nt;
-{
-  assert field_membership(nt, context_extend(ctx, x, S), st, t.t, t.l, T);
-  assert membership(nt-1, context_extend(ctx, x, S), st, t.t, t.l, decl_tm(t.l, T));
-  var nm' := lemma_substitution_preserves_membership(ctx, st, x, s, S, ns, t.t, t.l, decl_tm(t.l, T), nt-1);
-  assert membership(nm', ctx, st, tm_subst(x, s, t.t), tm_subst(x, s, t).l, decl_subst(x, s, decl_tm(t.l, T)));
-  assert field_membership(nm'+1, ctx, st, tm_subst(x, s, t.t), tm_subst(x, s, t).l, tp_subst(x, s, T));
-  assert field_membership(nm'+1, ctx, st, tm_subst(x, s, t).t, tm_subst(x, s, t).l, tp_subst(x, s, T));
-  assert typing(nm'+2, ctx, st, tm_subst(x, s, t), tp_subst(x, s, T));   
-  n' := nm'+2;
-  helper_assert_exists_typing(nm'-1, n', ctx, st, x, s, S, t, T);
-}
-ghost method helper_assert_exists_typing(maxn: nat, n': nat, ctx: context, st: store, x: nat, s: tm, S: tp, t: tm, T: tp)
-  requires typing(maxn+3, ctx, st, tm_subst(x, s, t), tp_subst(x, s, T));
-  requires maxn+3==n';
-  ensures typing(n', ctx, st, tm_subst(x, s, t), tp_subst(x, s, T));
-{
-}
-
-ghost method lemma_substitution_preserves_typing(ctx: context, st: store, x: nat, s: tm, S: tp, ns: nat, t: tm, T: tp, n: nat) returns (n': nat)
-  requires value(s);
-  requires typing(ns, Context([]), st, s, S);
-  requires context_lookup(ctx, x).None?;
-  requires env_well_typed(ctx, st);
-  requires typing(n, context_extend(ctx, x, S), st, t, T);
-  ensures typing(n', ctx, st, tm_subst(x, s, t), tp_subst(x, s, T));
-  decreases n;
-{
-  if (t.tm_var?) {
-    if (t.x==x) {
-      assert tm_subst(x, s, t)==s;
-      corollary_typable_empty__closed(ns, st, s, S);
-      lemma_context_invariance(ns, Context([]), ctx, st, s, S);
-      n' := ns;
-      assert typing(n', ctx, st, s, S);
-      assert typing(n', ctx, st, tm_subst(x, s, t), T);
-      lemma_not_fn__subst_idem(x, s, T);
-    } else {
-      n' := 0;
-      assert typing(n', ctx, st, t, T);
-      if (tp_fn(x, T)) {
-        var nwfe := lemma_typing__wfe(n', ctx, st, t, T);
-        lemma_free_in_context_wfe_type(x, nwfe, ctx, st, T);
-        assert context_lookup(ctx, x).Some?;
-        assert false;
-      } else {
-        lemma_not_fn__subst_idem(x, s, T);
-      }
-    }
-  } else if (t.tm_loc?) {
-    n' := 0;
-    assert typing(n', ctx, st, t, T);
-    if (tp_fn(x, T)) {
-      var nwfe := lemma_typing__wfe(n', ctx, st, t, T);
-      lemma_free_in_context_wfe_type(x, nwfe, ctx, st, T);
-      assert context_lookup(ctx, x).Some?;
-      assert false;
-    } else {
-      lemma_not_fn__subst_idem(x, s, T);
-    }
-  } else if (t.tm_sel?) {
-    n' := lemma_case_sel_substitution_preserves_typing(ctx, st, x, s, S, ns, t, T, n-1);
-  } else if (t.tm_msel?) {
-    // TODO
-    assume exists n'':nat :: typing(n'', ctx, st, tm_subst(x, s, t), tp_subst(x, s, T));
-    var n'':nat :| typing(n'', ctx, st, tm_subst(x, s, t), tp_subst(x, s, T));
-    n' := n'';
-  } else if (t.tm_new?) {
-    // TODO
-    assume exists n'':nat :: typing(n'', ctx, st, tm_subst(x, s, t), tp_subst(x, s, T));
-    var n'':nat :| typing(n'', ctx, st, tm_subst(x, s, t), tp_subst(x, s, T));
-    n' := n'';
-  } else {
-  }
-}
-ghost method helper_assert_membership(n: nat, ctx: context, s: store, t: tm, l: nat, d: decl, z: nat)
-  requires z == fresh_in_context(ctx);
-  requires membership(n, ctx, s, t, l, d);
-  ensures decl_label(d)==l &&
-  n>0 && exists T, T' :: typing(n-1, ctx, s, t, T') &&
-  subtype(n-1, ctx, s, T', T) &&
-  exists Ds ::
-  expansion(n-1, ctx, s, z, T, Ds) &&
-  ((Ds.decls_fin? &&
-     ((path(t) && T'==T && exists d' :: d' in lst2seq(Ds.decls) && d==decl_subst(z, t, d')) ||
-      (!path(t) && d in lst2seq(Ds.decls) && !decl_fn(z, d)))) ||
-   (Ds.decls_bot? && decl_bot(d)));
-{
-}
-ghost method lemma_fresh_equiv_membership(z: nat, z': nat, ctx: context, st: store, x: nat, s: tm, o: tm, l: nat, To: tp, To': tp, Ds': decls, d: decl, maxn: nat) returns (Ds'': decls)
-  requires decl_label(decl_subst(x, s, d))==l;
-  requires typing(maxn, ctx, st, tm_subst(x, s, o), tp_subst(x, s, To'));
-  requires subtype(maxn, ctx, st, tp_subst(x, s, To'), tp_subst(x, s, To));
-  requires expansion(maxn, ctx, st, z, tp_subst(x, s, To), Ds');
-  requires ((Ds'.decls_fin? &&
-     ((path(tm_subst(x, s, o)) && tp_subst(x, s, To')==tp_subst(x, s, To) && exists d'' :: d'' in lst2seq(Ds'.decls) && decl_subst(x, s, d)==decl_subst(z, tm_subst(x, s, o), d'')) ||
-      (!path(tm_subst(x, s, o)) && decl_subst(x, s, d) in lst2seq(Ds'.decls) && !decl_fn(z, decl_subst(x, s, d))))) ||
-   (Ds'.decls_bot? && decl_bot(decl_subst(x, s, d))));
-  requires value(s);
-  requires context_lookup(ctx, x).None?;
-  requires env_well_typed(ctx, st);
-  requires context_lookup(ctx, z).None?;
-  requires context_lookup(ctx, z').None?;
-  ensures expansion(maxn, ctx, st, z', tp_subst(x, s, To), Ds'');
-  ensures ((Ds''.decls_fin? &&
-     ((path(tm_subst(x, s, o)) && tp_subst(x, s, To')==tp_subst(x, s, To) && exists d'' :: d'' in lst2seq(Ds''.decls) && decl_subst(x, s, d)==decl_subst(z', tm_subst(x, s, o), d'')) ||
-      (!path(tm_subst(x, s, o)) && decl_subst(x, s, d) in lst2seq(Ds''.decls) && !decl_fn(z', decl_subst(x, s, d))))) ||
-   (Ds''.decls_bot? && decl_bot(decl_subst(x, s, d))));
-{
-  assume exists Ds''' ::  expansion(maxn, ctx, st, z', tp_subst(x, s, To), Ds''') &&
-   ((Ds'''.decls_fin? &&
-     ((path(tm_subst(x, s, o)) && tp_subst(x, s, To')==tp_subst(x, s, To) && exists d'' :: d'' in lst2seq(Ds'''.decls) && decl_subst(x, s, d)==decl_subst(z', tm_subst(x, s, o), d'')) ||
-      (!path(tm_subst(x, s, o)) && decl_subst(x, s, d) in lst2seq(Ds'''.decls) && !decl_fn(z', decl_subst(x, s, d))))) ||
-   (Ds'''.decls_bot? && decl_bot(decl_subst(x, s, d))));
-   var Ds''' :| expansion(maxn, ctx, st, z', tp_subst(x, s, To), Ds''') &&
-   ((Ds'''.decls_fin? &&
-     ((path(tm_subst(x, s, o)) && tp_subst(x, s, To')==tp_subst(x, s, To) && exists d'' :: d'' in lst2seq(Ds'''.decls) && decl_subst(x, s, d)==decl_subst(z', tm_subst(x, s, o), d'')) ||
-      (!path(tm_subst(x, s, o)) && decl_subst(x, s, d) in lst2seq(Ds'''.decls) && !decl_fn(z', decl_subst(x, s, d))))) ||
-   (Ds'''.decls_bot? && decl_bot(decl_subst(x, s, d))));
-   Ds'' := Ds''';
-}
-ghost method lemma_substitution_preserves_membership(ctx: context, st: store, x: nat, s: tm, S: tp, ns: nat, o: tm, l: nat, d: decl, nm: nat) returns (nm': nat)
-  requires value(s);
-  requires typing(ns, Context([]), st, s, S);
-  requires context_lookup(ctx, x).None?;
-  requires env_well_typed(ctx, st);
-  requires membership(nm, context_extend(ctx, x, S), st, o, l, d);
-  ensures  membership(nm', ctx, st, tm_subst(x, s, o), l, decl_subst(x, s, d));
-  decreases nm;
-{
-    var z:nat := fresh_in_context(context_extend(ctx, x, S));
-    helper_assert_membership(nm, context_extend(ctx, x, S), st, o, l, d, z);
-    assert decl_label(d)==l &&
-    nm>0 && exists To:tp, To':tp :: typing(nm-1, context_extend(ctx, x, S), st, o, To') &&
-    subtype(nm-1, context_extend(ctx, x, S), st, To', To) &&
-    exists Ds ::
-    expansion(nm-1, context_extend(ctx, x, S), st, z, To, Ds) &&
-    ((Ds.decls_fin? &&
-      ((path(o) && To'==To && exists d' :: d' in lst2seq(Ds.decls) && d==decl_subst(z, o, d')) ||
-       (!path(o) && d in lst2seq(Ds.decls) && !decl_fn(z, d)))) ||
-     (Ds.decls_bot? && decl_bot(d)));
-    var To:tp, To':tp, Ds:decls :| typing(nm-1, context_extend(ctx, x, S), st, o, To') &&
-    subtype(nm-1, context_extend(ctx, x, S), st, To', To) &&
-    expansion(nm-1, context_extend(ctx, x, S), st, z, To, Ds) &&
-    ((Ds.decls_fin? &&
-      ((path(o) && To'==To && exists d' :: d' in lst2seq(Ds.decls) && d==decl_subst(z, o, d')) ||
-       (!path(o) && d in lst2seq(Ds.decls) && !decl_fn(z, d)))) ||
-     (Ds.decls_bot? && decl_bot(d)));
-    var no' := lemma_substitution_preserves_typing(ctx, st, x, s, S, ns, o, To', nm-1);
-    var nos' := lemma_substitution_preserves_subtype(ctx, st, x, s, S, ns, To', To, nm-1);
-    var nox', Ds' := lemma_substitution_preserves_expansion(ctx, st, x, s, S, ns, z, To, Ds, nm-1);
-    assert typing(no', ctx, st, tm_subst(x, s, o), tp_subst(x, s, To'));
-    assert subtype(nos', ctx, st, tp_subst(x, s, To'), tp_subst(x, s, To));
-    assert expansion(nox', ctx, st, z, tp_subst(x, s, To), Ds');
-    assert decls_subst_p(x, s, Ds, Ds');
-    if (Ds.decls_fin?) {
-      assert Ds'.decls_fin?;
-      if (path(o)) {
-        lemma_path_subst(x, s, o);
-        assert path(tm_subst(x, s, o));
-        assert To'==To && exists d' :: d' in lst2seq(Ds.decls) && d==decl_subst(z, o, d');
-        assert tp_subst(x, s, To')==tp_subst(x, s, To);
-        var d' :| d' in lst2seq(Ds.decls) && d==decl_subst(z, o, d');
-        assert decl_subst(x, s, d') in lst2seq(Ds'.decls);
-        lemma_decl_subst2(x, s, z, o, d');
-        assert d==decl_subst(z, o, d');
-        assert decl_subst(x, s, d)==decl_subst(x, s, decl_subst(z, o, d'));
-        assert decl_subst(x, s, decl_subst(z, o, d'))==decl_subst(z, tm_subst(x, s, o), decl_subst(x, s, d'));
-        assert decl_subst(x, s, d)==decl_subst(z, tm_subst(x, s, o), decl_subst(x, s, d'));
-        assert path(tm_subst(x, s, o)) && tp_subst(x, s, To')==tp_subst(x, s, To) && decl_subst(x, s, d') in lst2seq(Ds'.decls) && decl_subst(x, s, d)==decl_subst(z, tm_subst(x, s, o), decl_subst(x, s, d'));
-        assert exists d'' :: d'' in lst2seq(Ds'.decls) && decl_subst(x, s, d)==decl_subst(z, tm_subst(x, s, o), d'');
-        assert (path(tm_subst(x, s, o)) && tp_subst(x, s, To')==tp_subst(x, s, To) && exists d'' :: d'' in lst2seq(Ds'.decls) && decl_subst(x, s, d)==decl_subst(z, tm_subst(x, s, o), d''));
-      } else {
-        assert !path(o);
-        lemma_not_path_subst(x, s, o);
-        assert !path(tm_subst(x, s, o));
-        assert d in lst2seq(Ds.decls) && !decl_fn(z, d);
-        assert decl_subst(x, s, d) in lst2seq(Ds'.decls);
-        lemma_decl_fn_subst(z, x, s, d);
-        assert !decl_fn(z, decl_subst(x, s, d));
-        assert !path(tm_subst(x, s, o)) && decl_subst(x, s, d) in lst2seq(Ds'.decls) && !decl_fn(z, decl_subst(x, s, d));
-      }
-    } else if (Ds.decls_bot?) {
-      assert Ds'.decls_bot?;
-      assert decl_bot(d);
-      lemma_decl_bot__subst_idem(x, s, d);
-      assert decl_bot(decl_subst(x, s, d));
-    } else {
-      assert false;
-    }
-    assert ((Ds'.decls_fin? &&
-      ((path(tm_subst(x, s, o)) && tp_subst(x, s, To')==tp_subst(x, s, To) && exists d' :: d' in lst2seq(Ds'.decls) && decl_subst(x, s, d)==decl_subst(z, tm_subst(x, s, o), d')) ||
-       (!path(tm_subst(x, s, o)) && decl_subst(x, s, d) in lst2seq(Ds'.decls) && !decl_fn(z, decl_subst(x, s, d))))) ||
-     (Ds'.decls_bot? && decl_bot(decl_subst(x, s, d))));
- 
-    var maxn := no';
-    if (maxn < nos') {
-      maxn := nos';
-    }
-    if (maxn < nox') {
-      maxn := nox';
-    }
-    lemma_typing_monotonic_plus(no', maxn, ctx, st, tm_subst(x, s, o), tp_subst(x, s, To'));
-    lemma_subtype_monotonic_plus(nos', maxn, ctx, st, tp_subst(x, s, To'), tp_subst(x, s, To));
-    lemma_expansion_monotonic_plus(nox', maxn, ctx, st, z, tp_subst(x, s, To), Ds');
-  assert decl_label(decl_subst(x, s, d))==l;
-  assert typing(maxn, ctx, st, tm_subst(x, s, o), tp_subst(x, s, To'));
-  assert subtype(maxn, ctx, st, tp_subst(x, s, To'), tp_subst(x, s, To));
-  assert expansion(maxn, ctx, st, z, tp_subst(x, s, To), Ds');
-  assert ((Ds'.decls_fin? &&
-     ((path(tm_subst(x, s, o)) && tp_subst(x, s, To')==tp_subst(x, s, To) && exists d'' :: d'' in lst2seq(Ds'.decls) && decl_subst(x, s, d)==decl_subst(z, tm_subst(x, s, o), d'')) ||
-      (!path(tm_subst(x, s, o)) && decl_subst(x, s, d) in lst2seq(Ds'.decls) && !decl_fn(z, decl_subst(x, s, d))))) ||
-   (Ds'.decls_bot? && decl_bot(decl_subst(x, s, d))));
-  var z':nat := fresh_in_context(ctx);
-  var Ds'' := lemma_fresh_equiv_membership(z, z', ctx, st, x, s, o, l, To, To', Ds', d, maxn);
-  assert expansion(maxn, ctx, st, z', tp_subst(x, s, To), Ds'');
-  assert ((Ds''.decls_fin? &&
-     ((path(tm_subst(x, s, o)) && tp_subst(x, s, To')==tp_subst(x, s, To) && exists d'' :: d'' in lst2seq(Ds''.decls) && decl_subst(x, s, d)==decl_subst(z', tm_subst(x, s, o), d'')) ||
-      (!path(tm_subst(x, s, o)) && decl_subst(x, s, d) in lst2seq(Ds''.decls) && !decl_fn(z', decl_subst(x, s, d))))) ||
-   (Ds''.decls_bot? && decl_bot(decl_subst(x, s, d))));
-  nm' := maxn + 1;
-  lemma_assert_membership'(maxn, nm', ctx, st, x, s, o, l, d, To, To', z', Ds'');
-}
-ghost method lemma_substitution_preserves_subtype(ctx: context, st: store, x: nat, s: tm, S: tp, ns: nat, T': tp, T: tp, n: nat) returns (n': nat)
-  requires value(s);
-  requires typing(ns, Context([]), st, s, S);
-  requires context_lookup(ctx, x).None?;
-  requires env_well_typed(ctx, st);
-  requires subtype(n, context_extend(ctx, x, S), st, T', T);
-  ensures subtype(n', ctx, st, tp_subst(x, s, T'), tp_subst(x, s, T));
-{
-  // TODO 
-  assume exists n'':nat :: subtype(n'', ctx, st, tp_subst(x, s, T'), tp_subst(x, s, T));
-  var n'':nat :| subtype(n'', ctx, st, tp_subst(x, s, T'), tp_subst(x, s, T));
-  n' := n'';
-}
-predicate decls_subst_p(x: nat, s: tm, Ds: decls, Ds': decls)
-  ensures decls_subst_p(x, s, Ds, Ds') ==> (Ds.decls_bot? <==> Ds'.decls_bot?);
-  ensures decls_subst_p(x, s, Ds, Ds') ==> (Ds.decls_fin? <==> Ds'.decls_fin?);
-{
-  match Ds
-  case decls_bot => Ds'.decls_bot?
-  case decls_fin(ds) => Ds'.decls_fin? && forall d :: d in lst2seq(Ds.decls) ==> decl_subst(x, s, d) in lst2seq(Ds'.decls)
-}
-ghost method lemma_substitution_preserves_expansion(ctx: context, st: store, x: nat, s: tm, S: tp, ns: nat, z: nat, T: tp, Ds: decls, n: nat) returns (n': nat, Ds': decls)
-  requires value(s);
-  requires typing(ns, Context([]), st, s, S);
-  requires context_lookup(ctx, x).None?;
-  requires context_lookup(ctx, z).None?;
-  requires env_well_typed(ctx, st);
-  requires expansion(n, context_extend(ctx, x, S), st, z, T, Ds);
-  ensures expansion(n', ctx, st, z, tp_subst(x, s, T), Ds');
-  ensures decls_subst_p(x, s, Ds, Ds');
-{
-  // TODO 
-  assume exists n'':nat, Ds'':decls :: decls_subst_p(x, s, Ds, Ds'') && expansion(n'', ctx, st, z, tp_subst(x, s, T), Ds'');
-  var n'':nat, Ds'':decls :| decls_subst_p(x, s, Ds, Ds'') && expansion(n'', ctx, st, z, tp_subst(x, s, T), Ds'');
-  n' := n'';
-  Ds' := Ds'';
-}
-
-ghost method lemma_substitution_preserves_typing_with_narrowing(ctx: context, st: store, x: nat, s: tm, S: tp, S': tp, ns: nat, nss: nat, t: tm, T: tp, n: nat) returns (n': nat, Ts: tp)
-  requires value(s);
-  requires typing(ns, Context([]), st, s, S);
-  requires context_lookup(ctx, x).None?;
-  requires env_well_typed(ctx, st);
-  requires subtype(nss, ctx, st, S, S');
-  requires typing(n, context_extend(ctx, x, S'), st, t, T);
-  ensures typing(n', ctx, st, tm_subst(x, s, t), Ts);
-  ensures subtype(n', ctx, st, Ts, tp_subst(x, s, T));
-  decreases n;
-{
-  if (t.tm_var?) {
-    if (t.x==x) {
-      assert tm_subst(x, s, t)==s;
-      corollary_typable_empty__closed(ns, st, s, S);
-      lemma_context_invariance(ns, Context([]), ctx, st, s, S);
-      assert typing(ns, ctx, st, s, S);
-      assert typing(ns, ctx, st, tm_subst(x, s, t), S);
-      assert typing(n, context_extend(ctx, x, S'), st, t, S');
-      assert S'==T;
-      var nwfe := lemma_subtype__wfe(nss, ctx, st, S, S');
-      lemma_wfe_type_not_in_context(x, nwfe, ctx, st, S');
-      lemma_not_fn__subst_idem(x, s, S');
-      assert tp_subst(x, s, S')==S';
-      Ts := S;
-      n' := ns;
-      if (n' < nss) {
-       n' := nss;
-      }
-      lemma_typing_monotonic_plus(ns, n', ctx, st, tm_subst(x, s, t), Ts);
-      lemma_subtype_monotonic_plus(nss, n', ctx, st, Ts, S');
-    } else {
-      assert tm_subst(x, s, t)==t;
-      assert typing(n, ctx, st, t, T);
-      var nwfe := lemma_typing__wfe(n, ctx, st, t, T);
-      lemma_wfe_type_not_in_context(x, nwfe, ctx, st, T);
-      lemma_not_fn__subst_idem(x, s, T);
-      Ts := T;
-      n' := n;
-      if (n' < nwfe+1) {
-        n' := nwfe+1;
-      }
-      lemma_typing_monotonic_plus(n, n', ctx, st, tm_subst(x, s, t), Ts);
-      lemma_subtype_monotonic_plus(nwfe+1, n', ctx, st, Ts, Ts);
-    }
-  } else if (t.tm_loc?) {
-    assert tm_subst(x, s, t)==t;
-    assert typing(n, ctx, st, t, T);
-    var nwfe := lemma_typing__wfe(n, ctx, st, t, T);
-    lemma_wfe_type_not_in_context(x, nwfe, ctx, st, T);
-    lemma_not_fn__subst_idem(x, s, T);
-    Ts := T;
-    n' := n;
-    if (n' < nwfe+1) {
-      n' := nwfe+1;
-    }
-    lemma_typing_monotonic_plus(n, n', ctx, st, tm_subst(x, s, t), Ts);
-    lemma_subtype_monotonic_plus(nwfe+1, n', ctx, st, Ts, Ts);
-  } else if (t.tm_sel?) {
-    // TODO
-    assume exists n'_:nat, Ts_:tp ::
-    typing(n'_, ctx, st, tm_subst(x, s, t), Ts_) &&
-    subtype(n'_, ctx, st, Ts_, tp_subst(x, s, T));
-    var n'_:nat, Ts_:tp :|
-    typing(n'_, ctx, st, tm_subst(x, s, t), Ts_) &&
-    subtype(n'_, ctx, st, Ts_, tp_subst(x, s, T)); 
-    n' := n'_;
-    Ts := Ts_;
-  } else if (t.tm_msel?) {
-    // TODO
-    assume exists n'_:nat, Ts_:tp ::
-    typing(n'_, ctx, st, tm_subst(x, s, t), Ts_) &&
-    subtype(n'_, ctx, st, Ts_, tp_subst(x, s, T));
-    var n'_:nat, Ts_:tp :|
-    typing(n'_, ctx, st, tm_subst(x, s, t), Ts_) &&
-    subtype(n'_, ctx, st, Ts_, tp_subst(x, s, T)); 
-    n' := n'_;
-    Ts := Ts_;
-  } else if (t.tm_new?) {
-    // TODO
-  assume exists n'_:nat, Ts_:tp ::
-    typing(n'_, ctx, st, tm_subst(x, s, t), Ts_) &&
-    subtype(n'_, ctx, st, Ts_, tp_subst(x, s, T));
-    var n'_:nat, Ts_:tp :|
-    typing(n'_, ctx, st, tm_subst(x, s, t), Ts_) &&
-    subtype(n'_, ctx, st, Ts_, tp_subst(x, s, T)); 
-    n' := n'_;
-    Ts := Ts_;
-  } else {
-  }
-}
-
-ghost method corollary_sanity_check_substitution_preserves_typing(ctx: context, st: store, x: nat, s: tm, S: tp, ns: nat, t: tm, T: tp, n: nat) returns (n': nat)
-  requires value(s);
-  requires typing(ns, Context([]), st, s, S);
-  requires context_lookup(ctx, x).None?;
-  requires env_well_typed(ctx, st);
-  requires typing(n, context_extend(ctx, x, S), st, t, T);
-  ensures typing(n', ctx, st, tm_subst(x, s, t), tp_subst(x, s, T));
-  decreases n;
-{
-  lemma_context_invariance(ns, Context([]), ctx, st, s, S);
-  var nss_ := lemma_typing__wfe(ns, ctx, st, s, S);
-  var n'_, Ts_ := lemma_substitution_preserves_typing_with_narrowing(ctx, st, x, s, S, S, ns, nss_+1, t, T, n);
-  assume Ts_ == tp_subst(x, s, T);
-  n' := n'_;
-}
-
-ghost method corollary_sanity_check_substitution_preserves_typing_with_narrowing(ctx: context, st: store, x: nat, s: tm, S: tp, S': tp, ns: nat, nss: nat, t: tm, T: tp, n: nat) returns (n': nat, Ts: tp)
-  requires value(s);
-  requires typing(ns, Context([]), st, s, S);
-  requires context_lookup(ctx, x).None?;
-  requires env_well_typed(ctx, st);
-  requires subtype(nss, ctx, st, S, S');
-  requires typing(n, context_extend(ctx, x, S'), st, t, T);
-  requires S==S';
-  ensures Ts==tp_subst(x, s, T);
-  ensures typing(n', ctx, st, tm_subst(x, s, t), Ts);
-  ensures subtype(n', ctx, st, Ts, tp_subst(x, s, T));
-  decreases n;
-{
-  Ts := tp_subst(x, s, T);
-  var n'_ := lemma_substitution_preserves_typing(ctx, st, x, s, S, ns, t, T, n);
-  var nss_ := lemma_typing__wfe(n'_, ctx, st, tm_subst(x, s, t), Ts);
-  n' := n'_;
-  if (n' < nss_+1) {
-    n' := nss_+1;
-  }
-  lemma_typing_monotonic_plus(n'_, n', ctx, st, tm_subst(x, s, t), Ts);
-  lemma_subtype_monotonic_plus(nss_+1, n', ctx, st, Ts, Ts);
-}
-
-ghost method theorem_preservation(ctx: context, st: store, t: tm, T: tp, nt: nat) returns (n: nat, T': tp, st': store, t': tm)
-  requires typing(nt, ctx, st, t, T);
-  requires step(t, st).Some?;
-  ensures step(t, st) == Some(P(t', st'));
-  ensures typing(n, ctx, st', t', T');
-  ensures subtype(n, ctx, st', T', T);
-{
-  t' := step(t, st).get.fst;
-  st' := step(t, st).get.snd;
-
-  assume exists n_:nat, T'_:tp ::
-  typing(n_, ctx, st', t', T'_) &&
-  subtype(n_, ctx, st', T'_, T);
-  var n_:nat, T'_:tp :|
-  typing(n_, ctx, st', t', T'_) &&
-  subtype(n_, ctx, st', T'_, T);
-  n := n_;
-  T' := T'_;
 }
